@prefix : <https://w3c.github.io/dxwg/profiledesc#> .
@prefix dc: <http://purl.org/dc/elements/1.1/> .
@prefix dct: <http://purl.org/dc/terms/> .
@prefix owl: <http://www.w3.org/2002/07/owl#> .
@prefix rdf: <http://www.w3.org/1999/02/22-rdf-syntax-ns#> .
@prefix xml: <http://www.w3.org/XML/1998/namespace> .
@prefix xsd: <http://www.w3.org/2001/XMLSchema#> .
@prefix dcat: <http://www.w3.org/ns/dcat#> .
@prefix foaf: <http://xmlns.com/foaf/0.1/> .
@prefix prov: <http://www.w3.org/ns/prov#> .
@prefix rdfs: <http://www.w3.org/2000/01/rdf-schema#> .
@prefix skos: <http://www.w3.org/2004/02/skos/core#> .
@prefix dcterms: <http://purl.org/dc/terms/> .
@base <https://w3c.github.io/dxwg/profiledesc> .

<https://w3c.github.io/dxwg/profiledesc> rdf:type owl:Ontology ;
                                          owl:versionIRI <https://w3c.github.io/dxwg/profiledesc/1.0> ;
                                          rdfs:label "Profile Descriptions Ontology" ;
                                          dcterms:contributor <http://orcid.org/0000-0002-8742-7730> ;
                                          dc:creator "Rob Atkinson" ;
                                          rdfs:comment """This ontology is for describing relationships between standards/specifications, profiles of them and supporting artefacts such as validating resources.

This model starts with [http://dublincore.org/2012/06/14/dcterms#Standard](dcterms:Standard) entities which can either be Base Specifications (a standard not profiling any other Standard) or Profiles (Standards which do profile others). Base Specifications or Profiles can have Implementation Resource Descriptors associated with them that defines implementing rules for the it. Implementation Resource Descriptors must indicate the role they play (to guide, to validate etc.) and the formalism they adhere to (dct:format) to allow for content negotiation. A vocabulary of Implementation Resource Roles are provided alongside this ontology but that list is extensible."""@en ;
                                          owl:versionInfo "1.0" ;
                                          dc:contributor "Nicholas Car" ,
                                                         "Simon Cox" ;
                                          dcterms:modified "2018-09-13"^^xsd:date ;
                                          dcterms:contributor <http://orcid.org/0000-0002-3884-3420> ;
                                          dcterms:created "2018-02-16"^^xsd:date .

#################################################################
#    Annotation properties
#################################################################

###  http://purl.org/dc/terms/conformsTo
dcterms:conformsTo rdf:type owl:AnnotationProperty ;
                   rdfs:subPropertyOf dc:relation ,
                                      dcterms:relation ;
                   rdfs:range dcterms:Standard .


###  http://purl.org/dc/terms/format
dcterms:format rdf:type owl:AnnotationProperty ;
               rdfs:subPropertyOf dc:format ;
               rdfs:range dcterms:MediaTypeOrExtent .


#################################################################
#    Object Properties
#################################################################

###  https://w3c.github.io/dxwg/profiledesc#artefact
:artefact
  rdf:type owl:ObjectProperty ;
  rdfs:comment "The artefact (resource) linked to a profile through an Implementation Resource Descriptor" ;
  rdfs:domain :ImplResourceDesc ;
  rdfs:label "artefact (resource) " ;
  skos:editorialNote "A property to link from a pd:ImplResourceDesc to the actual implementation resource. " ;
.

###  https://w3c.github.io/dxwg/profiledesc#hasProfile
:hasProfile rdf:type owl:ObjectProperty ;
            owl:inverseOf :profileOf ;
            rdfs:comment "A known profile of a specification."@en ;
            rdfs:label "has profile" .


###  https://w3c.github.io/dxwg/profiledesc#inheritedFrom
:inheritedFrom rdf:type owl:ObjectProperty ;
               rdfs:domain :ImplResourceDesc ;
               rdfs:range :Profile ;
               rdfs:comment "Provides a means to collate all inherited constraints from base specifications."@en ;
               skos:scopeNote "Profile from inheritance hierarchies defines these constraints. If absent, then the resource applies specifically to the profiles that refer to this resource."@en ;
               rdfs:label "inherited from" .


###  https://w3c.github.io/dxwg/profiledesc#profileOf
:profileOf rdf:type owl:ObjectProperty ;
           rdfs:domain :Profile ;
           rdfs:range :Profile ;
           skos:scopeNote "The semantics of the rdfs:Range means that any resource treated as a base specification can be regarded as a Profile (i.e. may be any specification with an empty set of additional constraints)."@en ;
           rdfs:comment "The immediate parent (base specification) an Implementation Profile describes conformance to."@en ;
           rdfs:label "profile of" .


###  https://w3c.github.io/dxwg/profiledesc#profileOfTransitive
:profileOfTransitive rdf:type owl:ObjectProperty ;
                     rdfs:domain :Profile ;
                     rdfs:range :Profile ;
                     skos:scopeNote "A means to list all the transitive hierarchy of base specifications that this Implementation Profile implies conformance to."@en ;
                     rdfs:comment "A base specification an Implementation Profile conforms to."@en ;
                     rdfs:label "transitive profile of" .


###  https://w3c.github.io/dxwg/profiledesc#resource
:resource rdf:type owl:ObjectProperty ;
          rdfs:range :ImplResourceDesc ;
          rdfs:comment "Link to an Implementation Resource Descriptor."@en ;
          rdfs:label "resource"@en .


###  https://w3c.github.io/dxwg/profiledesc#resourceRole
:resourceRole rdf:type owl:ObjectProperty ;
              rdfs:domain :ImplResourceDesc ;
              rdfs:range skos:Concept ;
              skos:scopeNote "Some roles are published alongside this ontology in a separate vocabulary."@en ;
              rdfs:comment "Functional role of an Implementation Resource."@en ;
              rdfs:label "resource role" .


###  https://w3c.github.io/dxwg/profiledesc#token
:token rdf:type owl:ObjectProperty ;
       rdfs:domain :Profile ;
       rdfs:range xsd:token .


#################################################################
#    Data properties
#################################################################

###  https://w3c.github.io/dxwg/profiledesc#token
:token rdf:type owl:DatatypeProperty .


#################################################################
#    Classes
#################################################################

###  https://w3c.github.io/dxwg/profiledesc#BaseSpecification
:BaseSpecification rdf:type owl:Class ;
                   rdfs:subClassOf :Profile ,
                                   [ rdf:type owl:Restriction ;
                                     owl:onProperty :profileOf ;
                                     owl:maxCardinality "0"^^xsd:nonNegativeInteger
                                   ] ;
                   rdfs:label "Base Specification" ;
                   skos:definition "A specification that defines all implementation constraints, without applying constraints on usage of another specification."@en ;
                   skos:scopeNote "This may not be a useful class: documents of any specification can be regarded as a trivial profile, so applications only need to be concerned with Profile conformance."@en .


###  https://w3c.github.io/dxwg/profiledesc#ImplResourceDesc
:ImplResourceDesc rdf:type owl:Class ;
                  rdfs:comment "A resource that defines implementing rules for a profile. Must indicate the purpose (dct:type) and the formalism (dct:format) used to allow machine mediation of such rules."@en ;
                  rdfs:label "Implementation Resource Descriptor"@en .


###  https://w3c.github.io/dxwg/profiledesc#ImplResourceRole
:ImplResourceRole rdf:type owl:Class ;
                  rdfs:subClassOf skos:Concept ;
                  rdfs:comment "The role that an Implementation Resource plays. Specific terms must come from a vocabulary."@en ;
                  rdfs:label "Implementation Resource Role" .


###  https://w3c.github.io/dxwg/profiledesc#Profile
:Profile rdf:type owl:Class ;
         rdfs:subClassOf dcterms:Standard ,
                         skos:Concept ;
         dc:source <https://www.w3.org/2017/dxwg/wiki/ProfileContext> ;
         rdfs:comment "Implementation Profile here is modelled as a skos:Concept to explicitly support the notion of profiles being organised as classification taxonomies. SKOS semantic relations such as skos:broader/narrower and broaderTransitive properties may be used."@en ;
         rdfs:label "Profile" ;
         skos:definition """A named set of constraints on one or more identified base specifications or other profiles, including the identification of any implementing subclasses of datatypes, semantic interpretations, vocabularies, options and parameters of those base specifications necessary to accomplish a particular function.

This definition includes what are often called \"application profiles\", \"metadata application profiles\", or \"metadata profiles\"."""@en .


#################################################################
#    Annotations
#################################################################

dcterms:conformsTo rdfs:isDefinedBy dcterms: ;
                   rdfs:comment "An established standard to which the described resource conforms."@en ;
                   rdfs:label "conforms to" .


:token rdfs:label "token" ;
       rdfs:comment "Short token for a profile.  For potential use in content negotiation. Will require a registry to disambiguate as do MIME type tokens."@en ,
                    "A short name identifying this profile for use in APIs. Avoids need for a global registry - APIs may need to have some concept of a namespace for tokens to disambiguate."@en .


###  Generated by the OWL API (version 4.2.8.20170104-2310) https://github.com/owlcs/owlapi
