@prefix dc: <http://purl.org/dc/elements/1.1/> .
@prefix dct: <http://purl.org/dc/terms/> .
@prefix owl: <http://www.w3.org/2002/07/owl#> .
@prefix rdf: <http://www.w3.org/1999/02/22-rdf-syntax-ns#> .
@prefix xsd: <http://www.w3.org/2001/XMLSchema#> .
@prefix dcat: <http://www.w3.org/ns/dcat#> .
@prefix prof: <https://w3c.github.io/dxwg/profiledesc#> .
@prefix prov: <http://www.w3.org/ns/prov#> .
@prefix rdfs: <http://www.w3.org/2000/01/rdf-schema#> .
@prefix dcterms: <http://purl.org/dc/terms/> .
@base <https://w3c.github.io/dxwg/profiledes> .

<https://w3c.github.io/dxwg/profiledesc_dcat_alignment.ttl> rdf:type owl:Ontology ;
                               owl:versionIRI <http://promsns.org/def/prof/1.0> ;
                               dcterms:contributor <http://orcid.org/0000-0002-8742-7730> ;
                               dc:description "This ontology defines an alignment with DCAT through subclassing relevant DCAT types and properties, without limiting the scope of the main profileDesc ontology to DCAT."@en ;
                               rdfs:label "Profile Description alignment to DCAT concepts"@en ;
                               owl:versionInfo "1.0"^^xsd:string ;
                               dc:creator "Rob Atkinson"^^xsd:string ;
                               dc:contributor "Nicholas Car"^^xsd:string ;
.

#################################################################
###  https://w3c.github.io/dxwg/profiledesc#hasProfile
prof:hasProfile rdf:type owl:ObjectProperty ;
                rdfs:comment "May be aligned as a subproperty of a (possible new) property for relationships between DCAT resources"@en ;
.

###  https://w3c.github.io/dxwg/profiledesc#profileOf
prof:profileOf rdf:type owl:ObjectProperty ;
               rdfs:domain prof:Profile ;
               rdfs:comment "May be aligned as a subproperty of a (possible new) property for relationships between DCAT resources"@en ;
.

###  https://w3c.github.io/dxwg/profiledesc#resource
prof:resource rdf:type owl:ObjectProperty ;
              rdfs:subPropertyOf dcat:distribution ;
.


###  https://w3c.github.io/dxwg/profiledesc#resourceRole
prof:resourceRole rdf:type owl:ObjectProperty ;
                  rdfs:comment "May be aligned as in future with DCAT distribution role qualification mechanisms"@en ;
.


###  http://purl.org/dc/terms/conformsTo
dcterms:conformsTo rdf:type owl:ObjectProperty ;
			             rdfs:comment "Alignment presumes that DCAT will also use this property to qualify profile conformance for distributions."@en ;
                   rdfs:range dcterms:Standard ;
.


###  http://purl.org/dc/terms/format
dcterms:format rdf:type owl:ObjectProperty ;
	             rdfs:comment "Alignment presumes that DCAT will also use this property to qualify profile conformance for distributions."@en ;
.


#################################################################
#    Classes
#################################################################


###  https://w3c.github.io/dxwg/profiledesc#ImplResourceDesc
prof:ImplResourceDesc rdf:type owl:Class ;
                      rdfs:comment "A resource that defines implementing rules for a profile. Must indicate the purpose (dct:type) and the formalism (dct:format) used to allow machine mediation of such rules."@en ;
                      rdfs:label "Implementation Resource Descriptor"@en ;
.


###  https://w3c.github.io/dxwg/profiledesc#ImplResourceRole
prof:ImplResourceRole rdf:type owl:Class ;
                      rdfs:subClassOf dcat:Distribution ;
                      rdfs:comment "Or a superclass of dcat:Distribution if dcat:Distribution domain remains dcat:Dataset"@en ;
.


###  https://w3c.github.io/dxwg/profiledesc#Profile
prof:Profile rdf:type owl:Class ;
             rdfs:subClassOf dcat:Resource ;
             rdfs:comment "This is a generic association"@en ;
.
