@prefix altp: <http://www.w3.org/ns/dx/conneg/altp#> .
@prefix dct: <http://purl.org/dc/terms/> .
@prefix owl: <http://www.w3.org/2002/07/owl#> .
@prefix rdf: <http://www.w3.org/1999/02/22-rdf-syntax-ns#> .
@prefix sdo: <http://schema.org/> .
@prefix xsd: <http://www.w3.org/2001/XMLSchema#> .
@prefix rdfs: <http://www.w3.org/2000/01/rdf-schema#> .
@prefix skos: <http://www.w3.org/2004/02/skos/core#> .

<http://www.w3.org/ns/dx/conneg/altp>
    a owl:Ontology ;
    rdfs:label "Alternative Profiles Ontology" ;
    rdfs:comment """This ontology allows for the description of representations of Internet resources.

Representations may conform to prof:Profile instances and may have the format of a particular dct:MediaType."""@en ;
    dct:created "2019-08-07"^^xsd:date ;
    dct:modified "2019-08-10"^^xsd:date ;
    dct:creator [
        a sdo:Person ;
        sdo:affiliation [
            sdo:name "SURROUND Australia Pty Ltd" ;
            sdo:url <https://surroundaustralia.com>
        ] ;
        sdo:email <mailto:nicholas.car@surroundaustralia.com> ;
        sdo:identifier <http://orcid.org/0000-0002-8742-7730> ;
        sdo:name "Nicholas J. Car"
    ] .

dct:conformsTo
    a owl:ObjectProperty ;
    rdfs:label "conforms to" ;
    dct:source dct:conformsTo ;
    skos:scopeNote "Use this property to indicate a dct:Standard that a altp:Representation conforms to." .

altp:hasRepresentation
    a owl:ObjectProperty ;
    rdfs:label "has representation" ;
    skos:definition "Indicates a Representation of a Resource."@en ;
    rdfs:domain rdf:Resource ;
    rdfs:range altp:Representation ;
    skos:scopeNote "Use this property to indicate a the HTTP-delivered representation of a resource." .

altp:hasDefaultRepresentation
    a owl:ObjectProperty ;
    rdfs:label "has default representation" ;
    skos:definition "Indicates the default Representation of a Resource."@en ;
    rdfs:subPropertyOf altp:hasRepresentation ;
    skos:scopeNote "Use this property to indicate the default HTTP-delivered representation of a resource that is obtained when no further instructions are given to a server to obtain a resource's representation other than the identification (URI) of the resource" .

rdf:Resource
    a owl:Class ;
    rdfs:label "Resource" ;
    skos:definition "The class resource, everything."@en ;
    rdfs:subClassOf [
        a owl:Restriction ;
        owl:onProperty altp:hasRepresentation ;
        owl:allValuesFrom altp:Representation
    ] ;
    dct:source "http://www.w3.org/2000/01/rdf-schema#Resource" ;
    skos:scopeNote "In the context of this mode, rdf:Resource instances are used to identify Internet resources, that is items identified by a URI." .

altp:Representation
    a owl:Class ;
    rdfs:label "Representation" ;
    skos:definition "An abstraction of the current or desired state of a thing in HTTP communications."@en ;
    rdfs:subClassOf [
        a owl:Restriction ;
        owl:onProperty dct:conformsTo ;
        owl:allValuesFrom dct:Standard
    ] ;
    dct:source <https://httpwg.org/specs/rfc7230.html> ;
    rdfs:isDefinedBy <http://www.w3.org/ns/dx/conneg/altp> ;
    skos:scopeNote "Use this class to indicate instances of representations of resources" .

dct:Standard
    a owl:Class ;
    rdfs:label "Standard" ;
    skos:definition "A basis for comparison; a reference point against which other things can be evaluated."@en ;
    dct:source "http://purl.org/dc/terms/Standard" ;
    skos:scopeNote "In the context of this mode, use this class to indicate instances of information models that representations of resources can conform to." .
