@prefix : <http://www.w3.org/ns/prof/roles/> .
@prefix dc: <http://purl.org/dc/elements/1.1/> .
@prefix dcat: <http://www.w3.org/ns/dcat#> .
@prefix dct: <http://purl.org/dc/terms/> .
@prefix dcterms: <http://purl.org/dc/terms/> .
@prefix foaf: <http://xmlns.com/foaf/0.1/> .
@prefix owl: <http://www.w3.org/2002/07/owl#> .
@prefix prof: <http://www.w3.org/ns/prof/> .
@prefix prov: <http://www.w3.org/ns/prov#> .
@prefix rdf: <http://www.w3.org/1999/02/22-rdf-syntax-ns#> .
@prefix rdfs: <http://www.w3.org/2000/01/rdf-schema#> .
@prefix skos: <http://www.w3.org/2004/02/skos/core#> .
@prefix xml: <http://www.w3.org/XML/1998/namespace> .
@prefix xsd: <http://www.w3.org/2001/XMLSchema#> .

:ConformanceTest a owl:NamedIndividual,
        skos:Concept,
        prof:ResourceRole ;
    skos:definition "Constraints specifying a conformance test"@en ;
    skos:prefLabel "Conformance Test Constraints"@en ;
    skos:topConceptOf : .

:FullConstraints a owl:NamedIndividual,
        skos:Concept,
        prof:ResourceRole ;
    skos:broader :Validation ;
    skos:definition "Complete set of constraints for a profile"@en ;
    skos:prefLabel "Full Constraints"@en .

:Guidance a owl:NamedIndividual,
        skos:Concept,
        prof:ResourceRole ;
    skos:definition "Guidance notes of profile"@en ;
    skos:prefLabel "Guidance"@en ;
    skos:topConceptOf : .

:PartConstraints a owl:NamedIndividual,
        skos:Concept,
        prof:ResourceRole ;
    skos:broader :Validation ;
    skos:definition "Partial set of constraints for a profile"@en ;
    skos:prefLabel "Part Constraints"@en .

:Specification a owl:NamedIndividual,
        skos:Concept,
        prof:ResourceRole ;
    skos:definition "Reference document which describes the standard"@en ;
    skos:prefLabel "Specification document"@en ;
    skos:topConceptOf : .

:Vocabulary a owl:NamedIndividual,
        skos:Concept,
        prof:ResourceRole ;
    skos:definition "Machine readable definition of a vocabulary or schema. Typically expressed in RDF, XSD, UML DDL, Table Schema or similar"@en ;
    skos:prefLabel "Vocabulary"@en ;
    skos:topConceptOf : .

:Validation a owl:NamedIndividual,
        skos:Concept,
        prof:ResourceRole ;
    skos:definition "Artifact that is used directly in validation, such as XSD, Schematron, SHACL, ShEx"@en ;
    skos:prefLabel "Validation"@en ;
    skos:topConceptOf : .

: a skos:ConceptScheme ;
    rdfs:label "Resource Roles vocabulary"@en ;
    dc:contributor "Nicholas Car",
        "Simon Cox" ;
    dc:creator "Rob Atkinson" ;
    dcterms:contributor <http://orcid.org/0000-0002-3884-3420>,
        <http://orcid.org/0000-0002-8742-7730> ;
    dcterms:created "2018-02-16"^^xsd:date ;
    dcterms:modified "2018-08-13"^^xsd:date ;
    rdfs:comment """A vocabulary of ResourceRole instances.

This vocabulary is both a SKOS vocabulary and also a list of instances of the Profile Ontology's ResourceRole class."""@en .
