# baseURI: http://www.w3.org/ns/dcat
# imports: http://purl.org/dc/terms/
# imports: http://www.w3.org/2004/02/skos/core
# imports: http://www.w3.org/ns/prov-o#
# prefix: dcat

@prefix dcat: <http://www.w3.org/ns/dcat#> .
@prefix dct: <http://purl.org/dc/terms/> .
@prefix dctype: <http://purl.org/dc/dcmitype/> .
@prefix foaf: <http://xmlns.com/foaf/0.1/> .
@prefix locn: <http://www.w3.org/ns/locn#> .
@prefix odrl: <http://www.w3.org/ns/odrl/2/> .
@prefix owl: <http://www.w3.org/2002/07/owl#> .
@prefix prov: <http://www.w3.org/ns/prov#> .
@prefix rdf: <http://www.w3.org/1999/02/22-rdf-syntax-ns#> .
@prefix rdfs: <http://www.w3.org/2000/01/rdf-schema#> .
@prefix sdo: <http://schema.org/> .
@prefix skos: <http://www.w3.org/2004/02/skos/core#> .
@prefix time: <http://www.w3.org/2006/time#> .
@prefix vcard: <http://www.w3.org/2006/vcard/ns#> .
@prefix xsd: <http://www.w3.org/2001/XMLSchema#> .

<http://www.w3.org/ns/dcat>
  rdf:type owl:Ontology ;
  dct:contributor [
      rdf:type foaf:Person ;
      rdfs:seeAlso <https://orcid.org/0000-0002-3884-3420> ;
      foaf:name "Simon J D Cox
	       
      foaf:workInfoHomepage <http://people.csiro.au/Simon-Cox> ;
      sdo:affiliation [
        foaf:homepage <https://csiro.au> ;
        foaf:name "Commonwealth Scientific and Industrial Research Organisation" ;
      ] ;
    ] ;
  dct:contributor [
      sdo:affiliation <http://www.w3.org/data#W3C> ;
      rdfs:seeAlso <http://philarcher.org/foaf.rdf#me> ;
      foaf:homepage <http://www.w3.org/People/all#phila> ;
      foaf:name "Phil Archer" ;
    ] ;
  dct:contributor [
      sdo:affiliation [
          foaf:homepage <http://ec.europa.eu/dgs/informatics/> ;
          foaf:name "European Commission, DG DIGIT" ;
        ] ;
      foaf:name "Vassilios Peristeras" ;
    ] ;
  dct:contributor [
      sdo:affiliation [
          foaf:homepage <http://okfn.org> ;
          foaf:name "Open Knowledge Foundation" ;
        ] ;
      foaf:name "Rufus Pollock" ;
    ] ;
  dct:contributor [
      sdo:affiliation [
          foaf:homepage <http://www.refinitiv.com> ;
          foaf:name "Refinitiv" ;
        ] ;
      foaf:name "David Browning" ;
    ] ;
  dct:contributor [
      rdfs:seeAlso <http://makxdekkers.com/makxdekkers.rdf#me> ;
      foaf:homepage <http://makxdekkers.com/> ;
      foaf:name "Makx Dekkers" ;
    ] ;
  dct:contributor [
      rdfs:seeAlso <http://www.eurecom.fr/~atemezin/gatemezing-foaf.rdf> ;
      foaf:name "Ghislain Auguste Atemezing" ;
    ] ;
  dct:contributor [
      rdfs:seeAlso <https://jakub.klímek.com/#me> ;
      foaf:homepage <https://jakub.klímek.com/> ;
      foaf:name "Jakub Klímek" ;
    ] ;
  dct:contributor [
      foaf:homepage <http://www.asahi-net.or.jp/~ax2s-kmtn/> ;
      foaf:name "Shuji Kamitsuna" ;
    ] ;
  dct:contributor [
      foaf:name "Alejandra Gonzalez-Beltran" ;
      foaf:homepage <https://agbeltran.github.io> ;
      rdfs:seeAlso <https://orcid.org/0000-0003-3499-8262> ;
      sdo:affiliation [
                foaf:homepage <http://stfc.ac.uk> ;
                foaf:name "Science and Technology Facilities Council, UK" ;
       ] ;
    ] ;
 dct:contributor [
      foaf:name "Riccardo Albertoni" ;
      foaf:homepage <http://www.imati.cnr.it/index.php/people/8-curricula/178-riccardo-albertoni> ;
      foaf:homepage <https://w3id.org/people/ralbertoni/>;
      rdfs:seeAlso <https://orcid.org/0000-0001-5648-2713> ;
    ] ;
  dct:contributor [
      foaf:name "Andrea Perego" ;
      foaf:homepage <http://www.andrea-perego.name/foaf/#me>;
      rdfs:seeAlso <https://orcid.org/0000-0001-9300-2694> ;
    ] ;
  dct:contributor [
      foaf:name "Boris Villazón-Terrazas" ;
    ] ;
  dct:contributor [
      foaf:name "Marios Meimaris" ;
    ] ;
  dct:contributor [
      foaf:name "Martin Alvarez-Espinar" ;
    ] ;
  dct:contributor [
      foaf:name "Richard Cyganiak" ;
    ] ;
  dct:creator [
      rdfs:seeAlso <http://fadmaa.me/foaf.ttl> ;
      foaf:name "Fadi Maali" ;
    ] ;
  dct:creator [
      foaf:name "John Erickson" ;
    ] ;
  dct:modified "2012-04-24"^^xsd:date ;
  dct:modified "2013-09-20"^^xsd:date ;
  dct:modified "2013-11-28"^^xsd:date ;
  dct:modified "2017-12-19"^^xsd:date ;
  dct:modified "2019" ;
  rdfs:comment "DCAT es un vocabulario RDF diseñado para facilitar la interoperabilidad entre catálogos de datos publicados en la Web. Utilizando DCAT para describir datos disponibles en catálogos se aumenta la posibilidad de que sean descubiertos y se permite que las aplicaciones consuman fácilmente los metadatos de varios catálogos."@es ;
  rdfs:comment """DCAT est un vocabulaire développé pour faciliter l'interopérabilité entre les jeux de données publiées sur le Web.
				En utilisant DCAT pour décrire les jeux de données dans les catalogues de données, les fournisseurs de données augmentent leur découverte et permettent
				que les applications facilement les métadonnées de plusieurs catalogues. Il permet en plus la publication décentralisée des catalogues et facilitent
				la recherche fédérée des données entre plusieurs sites. Les métadonnées DCAT aggrégées peuvent servir comme un manifeste pour faciliter la préservation digitale des ressources.
				DCAT est définie à l'adresse http://www.w3.org/TR/vocab-dcat/. Une quelconque version de ce document normatif et ce vocabulaire est une erreur dans ce vocabulaire"""@fr ;
  rdfs:comment """DCAT is an RDF vocabulary designed to facilitate interoperability between data catalogs published on the Web.
          By using DCAT to describe datasets in data catalogs, publishers increase discoverability and enable
          applications easily to consume metadata from multiple catalogs. It further enables decentralized
          publishing of catalogs and facilitates federated dataset search across sites. Aggregated DCAT metadata can
          serve as a manifest file to facilitate digital preservation.
          DCAT is defined at http://www.w3.org/TR/vocab-dcat/. Any variance between that normative
          document and this schema is an error in this schema."""@en ;
  rdfs:comment "DCAT je RDF slovník navržený pro zprostředkování interoperability mezi datovými katalogy publikovanými na Webu. Poskytovatelé dat používáním slovníku DCAT pro popis datových sad v datových katalozích zvyšují jejich dohledatelnost a umožňují aplikacím konzumovat metadata z více katalogů. Dále je umožňena decentralizovaná publikace katalogů a federované dotazování na datové sady napříč katalogy. Agregovaná DCAT metadata mohou také sloužit jako průvodka umožňující digitální uchování informace. DCAT je definován na http://www.w3.org/TR/vocab-dcat/. Jakýkoliv nesoulad mezi odkazovaným dokumentem a tímto schématem je chybou v tomto schématu."@cs ;
  rdfs:comment "DCAT è un vocabolario RDF progettato per facilitare l'interoperabilità tra i cataloghi di dati pubblicati nel Web. Utilizzando DCAT per descrivere i dataset nei cataloghi di dati, i fornitori migliorano la capacità di individuazione dei dati e abilitano le  applicazioni al consumo di dati provenienti da cataloghi differenti. DCAT permette di decentralizzare la pubblicazione di cataloghi e facilita la ricerca federata dei dataset. L'aggregazione dei metadati federati può fungere da file manifesto per facilitare la conservazione digitale. DCAT è definito all'indirizzo http://www.w3.org/TR/vocab-dcat/. Qualsiasi scostamento tra tale definizione normativa e questo schema è da considerarsi un errore di questo schema."@it ;
  rdfs:comment """DCATは、ウェブ上で公開されたデータ・カタログ間の相互運用性の促進を目的とするRDFの語彙です。このドキュメントでは、その利用のために、スキーマを定義し、例を提供します。
データ・カタログ内のデータセットを記述するためにDCATを用いると、公開者が、発見可能性を増加させ、アプリケーションが複数のカタログのメタデータを容易に利用できるようになります。さらに、カタログの分散公開を可能にし、複数のサイトにまたがるデータセットの統合検索を促進します。集約されたDCATメタデータは、ディジタル保存を促進するためのマニフェスト・ファイルとして使用できます。"""@ja ;
  rdfs:comment """Το DCAT είναι ένα RDF λεξιλόγιο που σχεδιάσθηκε για να κάνει εφικτή τη διαλειτουργικότητα μεταξύ καταλόγων δεδομένων στον Παγκόσμιο Ιστό.
          Χρησιμοποιώντας το DCAT για την περιγραφή συνόλων δεδομένων, οι εκδότες αυτών αυξάνουν την ανακαλυψιμότητα και επιτρέπουν στις εφαρμογές την εύκολη κατανάλωση μεταδεδομένων από πολλαπλούς καταλόγους.
          Επιπλέον, δίνει τη δυνατότητα για αποκεντρωμένη έκδοση και διάθεση καταλόγων και επιτρέπει δυνατότητες ενοποιημένης αναζήτησης μεταξύ διαφορετικών πηγών.
          Συγκεντρωτικά μεταδεδομένα που έχουν περιγραφεί με το DCAT μπορούν να χρησιμοποιηθούν σαν ένα δηλωτικό αρχείο (manifest file) ώστε να διευκολύνουν την ψηφιακή συντήρηση."""@el ;
  rdfs:comment "هي أنطولوجية تسهل تبادل البيانات بين مختلف الفهارس على الوب. استخدام هذه الأنطولوجية يساعد على اكتشاف قوائم  البيانات المنشورة على الوب و يمكن التطبيقات المختلفة من الاستفادة أتوماتيكيا من البيانات المتاحة من مختلف الفهارس."@ar ;
  rdfs:label "El vocabulario de catálogo de datos"@es ;
  rdfs:label "Il vocabolario del catalogo dei dati"@it ;
  rdfs:label "Le vocabulaire des jeux de données "@fr ;
  rdfs:label "Slovník pro datové katalogy"@cs ;
  rdfs:label "The data catalog vocabulary"@en ;
  rdfs:label "Το λεξιλόγιο των καταλόγων δεδομένων"@el ;
  rdfs:label "أنطولوجية فهارس قوائم البيانات"@ar ;
  rdfs:label "データ・カタログ語彙（DCAT）"@ja ;
  owl:imports dct: ;
  owl:imports <http://www.w3.org/2004/02/skos/core> ;
  owl:imports <http://www.w3.org/ns/prov-o#> ;
  owl:versionInfo """Esta es una copia del vocabulario DCAT v1.0 disponible en https://www.w3.org/ns/dcat.ttl
con modificaciones en progreso para la nueva versión de DCAT que resultará del grupo 'W3C Data Exchange Working Group'"""@es ;
  owl:versionInfo """This is an updated copy of v1.0 of the DCAT vocabulary, taken from https://www.w3.org/ns/dcat.ttl and will replace that file when DCAT2 is published
Temporarily added imports for DCTerms, SKOS, FOAF to assist in development of v1.* or v2.0 by W3C Data Exchange Working Group"""@en ;
  owl:versionInfo """Toto je aktualizovaná kopie slovníku DCAT verze 1.0, převzatá z https://www.w3.org/ns/dcat.ttl a tento soubor po vydání DCAT2 nahradí. Dočasně jsou přidány importy pro DCTerms, SKOS, FOAF pro pomoc ve vývojei v1.* či v2.0 skupinou W3C Data Exchange Working Group"""@cs ;
  skos:editorialNote "English language definitions updated in this revision in line with ED. Multilingual text unevenly updated."@en ;
  foaf:maker [
      foaf:homepage <http://www.w3.org/2011/gld/> ;
      foaf:name "Government Linked Data WG" ;
    ] ;
  dct:license <https://www.w3.org/Consortium/Legal/2015/copyright-software-and-document>;
.
dcat:Catalog
  rdf:type rdfs:Class ;
  rdf:type owl:Class ;
  rdfs:comment "A curated collection of metadata about datasets and data services"@en ;
  rdfs:comment "Una colección seleccionada de metadatos sobre conjuntos de datos o servicios de datos"@es ;
  rdfs:comment "Una raccolta curata di metadati sui dataset e relativi servizi"@it ;
  rdfs:comment "Une collection élaborée de métadonnées sur les jeux de données"@fr ;
  rdfs:comment "Řízená kolekce metadat o datových sadách a datových službách"@cs ;
  rdfs:comment "Μια επιμελημένη συλλογή μεταδεδομένων περί συνόλων δεδομένων"@el ;
  rdfs:comment "مجموعة من توصيفات قوائم البيانات"@ar ;
  rdfs:comment "データ・カタログは、データセットに関するキュレートされたメタデータの集合です。"@ja ;
  rdfs:isDefinedBy <http://www.w3.org/TR/vocab-dcat/> ;
  rdfs:label "Catalog"@en ;
  rdfs:label "Catalogo"@it ;
  rdfs:label "Catalogue"@fr ;
  rdfs:label "Catálogo"@es ;
  rdfs:label "Katalog"@cs ;
  rdfs:label "Κατάλογος"@el ;
  rdfs:label "فهرس قوائم البيانات"@ar ;
  rdfs:label "カタログ"@ja ;
  rdfs:subClassOf dcat:Dataset ;
  rdfs:subClassOf [
      rdf:type owl:Restriction ;
      owl:allValuesFrom dcat:Resource ;
      owl:onProperty dct:hasPart ;
    ] ;
  skos:editorialNote "English, Italian, Spanish definitions updated in this revision. Multilingual text not yet updated."@en ;
  skos:scopeNote "A web-based data catalog is typically represented as a single instance of this class."@en ;
  skos:scopeNote "Normalmente, un catalogo di dati nel web viene rappresentato come una singola istanza di questa classe."@it ;
  skos:scopeNote "Normalmente, un catálogo de datos disponible en la web se representa como una única instancia de esta clase."@es ;
  skos:scopeNote "Webový datový katalog je typicky reprezentován jako jedna instance této třídy."@cs ;
  skos:scopeNote "Συνήθως, ένας κατάλογος δεδομένων στον Παγκόσμιο Ιστό αναπαρίσταται ως ένα στιγμιότυπο αυτής της κλάσης."@el ;
  skos:scopeNote "通常、ウェブ・ベースのデータ・カタログは、このクラスの1つのインスタンスとして表わされます。"@ja ;
.
dcat:CatalogRecord
  rdf:type rdfs:Class ;
  rdf:type owl:Class ;
  rdfs:comment "1つのデータセットを記述したデータ・カタログ内のレコード。"@ja ;
  rdfs:comment "A record in a data catalog, describing the registration of a single dataset or data service."@en ;
  rdfs:comment "Un record in un catalogo di dati che descrive un singolo dataset."@it ;
  rdfs:comment "Un registre du catalogue ou une entrée du catalogue, décrivant un seul jeu de données"@fr ;
  rdfs:comment "Un registro en un catálogo de datos que describe un solo conjunto de datos o un servicio de datos."@es ;
  rdfs:comment "Záznam v datovém katalogu popisující jednu datovou sadu či datovou službu."@cs ;
  rdfs:comment "Μία καταγραφή ενός καταλόγου, η οποία περιγράφει ένα συγκεκριμένο σύνολο δεδομένων."@el ;
  rdfs:isDefinedBy <http://www.w3.org/TR/vocab-dcat/> ;
  rdfs:label "Catalog Record"@en ;
  rdfs:label "Record di catalogo"@it ;
  rdfs:label "Registre du catalogue"@fr ;
  rdfs:label "Registro del catálogo"@es ;
  rdfs:label "Katalogizační záznam"@cs ;
  rdfs:label "Καταγραφή καταλόγου"@el ;
  rdfs:label "سجل"@ar ;
  rdfs:label "カタログ・レコード"@ja ;
  rdfs:subClassOf [
      rdf:type owl:Restriction ;
      owl:allValuesFrom dcat:Resource ;
      owl:onProperty foaf:primaryTopic ;
    ] ;
  rdfs:subClassOf [
      rdf:type owl:Restriction ;
      owl:cardinality "1"^^xsd:nonNegativeInteger ;
      owl:onProperty foaf:primaryTopic ;
    ] ;
  skos:editorialNote "English definition updated in this revision. Multilingual text not yet updated except the Spanish one and the Czech one."@en ;
  skos:scopeNote """This class is optional and not all catalogs will use it. It exists for
              catalogs where a distinction is made between metadata about a dataset or data service and
              metadata about the entry for the dataset or data service in the catalog. For example, the publication
              date property of the dataset reflects the date when the information was originally
              made available by the publishing agency, while the publication date of the catalog
              record is the date when the dataset was added to the catalog. In cases where both
              dates differ, or where only the latter is known, the publication date should only
              be specified for the catalog record. Notice that the W3C PROV Ontology allows
              describing further provenance information such as the details of the process and the
              agent involved in a particular change to a dataset."""@en ;
  skos:scopeNote """Esta clase es opcional y no todos los catálogos la utilizarán. Esta clase existe para catálogos
  				   que hacen una distinción entre los metadatos acerca de un conjunto de datos o un servicio de datos
  				   y los metadatos acerca de una entrada en ese conjunto de datos en el catálogo.
  				   Por ejemplo, la propiedad sobre la fecha de la publicación de los datos refleja la fecha en que la
  				   información fue originalmente publicada, mientras que la fecha de publicación del registro del catálogo
  				   es la fecha en que los datos se agregaron al mismo. En caso en que ambas fechas fueran diferentes, o en que sólo la
  				   fecha de publicación del registro del catálogo estuviera disponible, sólo debe especificarse en el registro del catálogo.
  				   Tengan en cuenta que la ontología PROV de W3C permite describir otra información sobre la proveniencia de los datos,
  				   como por ejemplo detalles del proceso y de los agentes involucrados en algún cambio específico a los datos."""@es ;
  skos:scopeNote """C'est une classe facultative et tous les catalogues ne l'utiliseront pas. Cette classe existe pour les catalogues
						ayant une distinction entre les métadonnées sur le jeu de données et les métadonnées sur une entrée du jeu de données dans le catalogue. """@fr ;
  skos:scopeNote "Questa classe è opzionale e non tutti i cataloghi la utilizzeranno. Esiste per cataloghi in cui si opera una distinzione tra i metadati relativi al dataset ed i metadati relativi alla gestione del dataset nel catalogo. Ad esempio, la  proprietà per indicare la data di pubblicazione del dataset rifletterà la data in cui l'informazione è stata originariamente messa a disposizione dalla casa editrice, mentre la data di pubblicazione per il record nel catalogo rifletterà la data in cui il dataset è stato aggiunto al catalogo. Nei casi dove solo quest'ultima sia nota, si utilizzerà esclusivamente la data di  pubblicazione relativa al record del catalogo. Si noti che l'Ontologia W3C PROV permette di descrivere ulteriori informazioni sulla provenienza, quali i dettagli del processo, la procedura e l'agente coinvolto in una particolare modifica di un dataset."@it ;
  skos:scopeNote "Tato třída je volitelná a ne všechny katalogy ji využijí. Existuje pro katalogy, ve kterých se rozlišují metadata datové sady či datové služby a metadata o záznamu o datové sadě či datové službě v katalogu. Například datum publikace datové sady odráží datum, kdy byla datová sada původně zveřejněna poskytovatelem dat, zatímco datum publikace katalogizačního záznamu je datum zanesení datové sady do katalogu. V případech kdy se obě data liší, nebo je známo jen to druhé, by mělo být specifikováno jen datum publikace katalogizačního záznamu. Všimněte si, že ontologie W3C PROV umožňuje popsat další informace o původu jako například podrobnosti o procesu konkrétní změny datové sady a jeho účastnících."@cs ;
  skos:scopeNote """Αυτή η κλάση είναι προαιρετική και δεν χρησιμοποιείται από όλους τους καταλόγους. Υπάρχει για τις περιπτώσεις καταλόγων όπου
					  γίνεται διαχωρισμός μεταξύ των μεταδεδομένων για το σύνολο των δεδομένων και των μεταδεδομένων για την καταγραφή του συνόλου δεδομένων εντός του καταλόγου.
					  Για παράδειγμα, η ιδιότητα της ημερομηνίας δημοσίευσης του συνόλου δεδομένων δείχνει την ημερομηνία κατά την οποία οι πληροφορίες έγιναν διαθέσιμες από τον φορέα δημοσίευσης,
					  ενώ η ημερομηνία δημοσίευσης της καταγραφής του καταλόγου δείχνει την ημερομηνία που το σύνολο δεδομένων προστέθηκε στον κατάλογο.
					  Σε περιπτώσεις που οι δύο ημερομηνίες διαφέρουν, ή που μόνο η τελευταία είναι γνωστή, η ημερομηνία δημοσίευσης θα πρέπει να δίνεται για την καταγραφή του καταλόγου.
					  Να σημειωθεί πως η οντολογία W3C PROV επιτρέπει την περιγραφή επιπλέον πληροφοριών ιστορικού όπως λεπτομέρειες για τη διαδικασία και τον δράστη που εμπλέκονται σε μία συγκεκριμένη αλλαγή εντός του συνόλου δεδομένων."""@el ;
  skos:scopeNote "このクラスはオプションで、すべてのカタログがそれを用いるとは限りません。これは、データセットに関するメタデータとカタログ内のデータセットのエントリーに関するメタデータとで区別が行われるカタログのために存在しています。例えば、データセットの公開日プロパティーは、公開機関が情報を最初に利用可能とした日付を示しますが、カタログ・レコードの公開日は、データセットがカタログに追加された日付です。両方の日付が異っていたり、後者だけが分かっている場合は、カタログ・レコードに対してのみ公開日を指定すべきです。W3CのPROVオントロジー[prov-o]を用いれば、データセットに対する特定の変更に関連するプロセスやエージェントの詳細などの、さらに詳しい来歴情報の記述が可能となることに注意してください。"@ja ;
.

dcat:DataService
  rdf:type owl:Class ;
  rdfs:comment "A site or end-point providing operations related to the discovery of, access to, or processing functions on, data or related resources."@en ;
  rdfs:comment "Un sitio o end-point que provee operaciones relacionadas a funciones de descubrimiento, acceso, o procesamiento de datos o recursos relacionados."@es ;
  rdfs:comment "Un sito o end-point che fornisce operazioni relative alla scoperta, all'accesso o all'elaborazione di funzioni su dati o risorse correlate."@it;
  rdfs:comment "Umístění či přístupový bod poskytující operace související s hledáním, přistupem k, či výkonem funkcí na datech či souvisejících zdrojích"@cs ;
  rdfs:label "Data service"@en ;
  rdfs:label "Servicio de datos"@es ;
  rdfs:subClassOf dctype:Service ;
  rdfs:subClassOf dcat:Resource ;
  rdfs:subClassOf [
      rdf:type owl:Restriction ;
      owl:maxCardinality "1"^^xsd:nonNegativeInteger ;
      owl:onProperty dcat:endpointURL ;
    ] ;
  skos:changeNote "New class added in DCAT 2.0."@en ;
  skos:changeNote "Nueva clase añadida en DCAT 2.0."@es ;
  skos:changeNote "Nuova classe aggiunta in DCAT 2.0."@it ;
  skos:changeNote "Nová třída přidaná ve verzi DCAT 2.0"@cs ;
  skos:scopeNote "The kind of service can be indicated using the dct:type property. Its value may be taken from a controlled vocabulary such as the INSPIRE spatial data service type vocabulary"@en ;
  skos:scopeNote "El tipo de servicio puede indicarse usando la propiedad dct:type. Su valor puede provenir de un vocabulario controlado, como por ejemplo el vocabulario de servicios de datos espaciales de INSPIRE."@es ;
  skos:scopeNote "Il tipo di servizio può essere indicato usando la proprietà dct:type. Il suo valore può essere preso da un vocabolario controllato come il vocabolario dei tipi di servizi per dati spaziali  di INSPIRE."@it ;
  skos:scopeNote "Druh služby může být indikován vlastností dct:type. Její hodnota může být z řízeného slovníku, kterým je například slovník typů prostorových datových služeb INSPIRE."@cs ;
  skos:scopeNote "If a dcat:DataService is bound to one or more specified Datasets, they are indicated by the dcat:servesDataset property."@en ;
  skos:scopeNote "Si un dcat:DataService está asociado con uno o más conjuntos de datos especificados, dichos conjuntos de datos pueden indicarse con la propiedad dcat:servesDataset."@es ;
  skos:scopeNote "Se un dcat:DataService è associato a uno o più Dataset specificati, questi sono indicati dalla proprietà dcat:serveDataset."@it ;
  skos:scopeNote "Pokud je dcat:DataService navázána na jednu či více Datových sad, jsou tyto indikovány vlstností dcat:servesDataset."@cs ;
.

dcat:Dataset
  rdf:type rdfs:Class ;
  rdf:type owl:Class ;
  rdfs:comment "1つのエージェントによって公開またはキュレートされ、1つ以上の形式でアクセスまたはダウンロードできるデータの集合。"@ja ;
  rdfs:comment "A collection of data, published or curated by a single source, and available for access or download in one or more represenations"@en ;
  rdfs:comment "Kolekce dat poskytovaná či řízená jedním zdrojem, která je k dispozici pro přístup či stažení v jednom či více formátech"@cs ;
  rdfs:comment "Raccolta di dati, pubblicati o curati da un'unica fonte, disponibili per l'accesso o il download in uno o più formati."@it ;
  rdfs:comment "Una colección de datos, publicados o conservados por una única fuente, y disponibles para ser accedidos o descargados en uno o más formatos"@es ;
  rdfs:comment "Une collection de données, publiée ou élaborée par une seule source, et disponible pour accès ou téléchargement dans un ou plusieurs formats"@fr ;
  rdfs:comment "Μία συλλογή από δεδομένα, δημοσιευμένη ή επιμελημένη από μία και μόνο πηγή, διαθέσιμη δε προς πρόσβαση ή μεταφόρτωση σε μία ή περισσότερες μορφές"@el ;
  rdfs:comment "قائمة بيانات منشورة أو مجموعة من قبل مصدر ما و متاح الوصول إليها أو تحميلها"@ar ;
  rdfs:isDefinedBy <http://www.w3.org/TR/vocab-dcat/> ;
  rdfs:label "Conjunto de datos"@es ;
  rdfs:label "Dataset"@en ;
  rdfs:label "Dataset"@it ;
  rdfs:label "Datová sada"@cs ;
  rdfs:label "Jeu de données"@fr ;
  rdfs:label "Σύνολο Δεδομένων"@el ;
  rdfs:label "قائمة بيانات"@ar ;
  rdfs:label "データセット"@ja ;
  rdfs:subClassOf dcat:Resource ;
  skos:changeNote "2018-02 - subclass of dctype:Dataset removed because scope of dcat:Dataset includes several other types from the dctype vocabulary."@en ;
  skos:changeNote "2018-02 - se eliminó el axioma de subclase con dctype:Dataset porque el alcance de dcat:Dataset incluye muchos otros tipos del vocabulario dctype."@es ;
  skos:changeNote "2018-02 - odstraněno tvrzení o podtřídě dctype:Dataset, jelikož rozsah dcat:Dataset zahrnuje několik dalších typů ze slovníku dctype."@cs ;
  skos:scopeNote """Cette classe représente le jeu de données publié par le fournisseur de données. Dans les cas où une distinction est nécessaire entre le jeu de donénes et son
					  entrée dans le catalogue, la classe registre de données peut être utilisée pour ce dernier. """@fr ;
  skos:scopeNote """Esta clase representa el conjunto de datos publicados. En los casos donde es necesario distinguir entre el
					conjunto de datos y su entrada en el catálogo de datos, se debe utilizar la clase 'registro del catálogo'."""@es ;
  skos:scopeNote "Questa classe rappresenta il dataset come pubblicato dall’editore. Nel caso in cui sia necessario operare  una distinzione fra i metadati originali del dataset e il record dei metadati ad esso associato nel catalogo (ad esempio, per distinguere la data di modifica del dataset da quella del dataset nel catalogo) si può impiegare la classe catalog record."@it ;
  skos:scopeNote "Tato třída reprezentuje datovou sadu tak, jak je publikována poskytovatelem dat. V případě potřeby rozlišení datové sady a jejího katalogizačního záznamu (jelikož metadata jako datum modifikace se mohou lišit) pro něj může být použita třída \"katalogizační záznam\"."@cs ;
  skos:scopeNote "This class describes the conceptual dataset. One or more representations might be available, with differing schematic layouts and formats or serializations."@en ;
  skos:scopeNote """This class represents the actual dataset as published by the dataset provider. In
          cases where a distinction between the actual dataset and its entry in the catalog is
          necessary (because metadata such as modification date and maintainer might differ), the
          catalog record class can be used for the latter."""@en ;
  skos:scopeNote """Η κλάση αυτή αναπαριστά το σύνολο δεδομένων αυτό καθ'εαυτό, όπως έχει δημοσιευθεί από τον εκδότη.
          Σε περιπτώσεις όπου είναι απαραίτητος ο διαχωρισμός μεταξύ του συνόλου δεδομένων και της καταγραφής αυτού στον κατάλογο (γιατί μεταδεδομένα όπως η ημερομηνία αλλαγής και ο συντηρητής μπορεί να διαφέρουν)
          η κλάση της καταγραφής καταλόγου μπορεί να χρησιμοποιηθεί για το τελευταίο."""@el ;
  skos:scopeNote "このクラスは、データセットの公開者が公開する実際のデータセットを表わします。カタログ内の実際のデータセットとそのエントリーとの区別が必要な場合（修正日と維持者などのメタデータが異なるかもしれないので）は、後者にcatalog recordというクラスを使用できます。"@ja ;
.
dcat:Distribution
  rdf:type rdfs:Class ;
  rdf:type owl:Class ;
  rdfs:comment """A specific representation of a dataset. A dataset might be available in multiple serializations that may differ in various ways,
                  including natural language, media-type or format, schematic organization, temporal and spatial resolution, level of detail or
                  profiles (which might specify any or all of the above)."""@en ;
  rdfs:comment """Una representación específica de los datos. Cada conjunto de datos puede estar disponible en
                  formas diferentes, las cuáles pueden variar en distintas formas, incluyendo el idioma,
                  'media-type' o formato, organización esquemática, resolución temporal y espacial, nivel de detalle o perfiles (que pueden especificar cualquiera o todas las diferencias anteriores)."""@es ;
  rdfs:comment "Rappresenta una forma disponibile e specifica del dataset. Ciascun dataset può essere disponibile in forme differenti, che possono rappresentare formati diversi o diversi punti di accesso per un dataset. Esempi di distribuzioni sono un file CSV scaricabile, una API o un RSS feed."@it ;
  rdfs:comment "Konkrétní reprezentace datové sady. Datová sada může být dostupná v různých serializacích, které se mohou navzájem lišit různými způsoby, mimo jiné přirozeným jazykem, media-typem či formátem, schematickou organizací, časovým a prostorovým rozlišením, úrovní detailu či profily (které mohou specifikovat některé či všechny tyto rozdíly)."@cs ;
  rdfs:comment """Représente une forme spécifique d'un jeu de données. Caque jeu de données peut être disponible
					sous différentes formes, celles-ci pouvant représenter différents formats du jeu de données ou différents endpoint. Des exemples de distribution
					sont des fichirs CSV, des API ou des flux RSS."""@fr ;
  rdfs:comment """Αναπαριστά μία συγκεκριμένη διαθέσιμη μορφή ενός συνόλου δεδομένων. Κάθε σύνολο δεδομενων μπορεί να είναι διαθέσιμο σε
					διαφορετικές μορφές, οι μορφές αυτές μπορεί να αναπαριστούν διαφορετικές μορφές αρχείων ή διαφορετικά σημεία διάθεσης.
					Παραδείγματα διανομών συμπεριλαμβάνουν ένα μεταφορτώσιμο αρχείο μορφής CSV, ένα API ή ένα RSS feed."""@el ;
  rdfs:comment "شكل محدد لقائمة البيانات يمكن الوصول إليه. قائمة بيانات ما يمكن أن تكون متاحه باشكال و أنواع متعددة.  ملف يمكن تحميله أو واجهة برمجية يمكن من خلالها الوصول إلى البيانات هي أمثلة على ذلك."@ar ;
  rdfs:comment "データセットの特定の利用可能な形式を表わします。各データセットは、異なる形式で利用できることがあり、これらの形式は、データセットの異なる形式や、異なるエンドポイントを表わす可能性があります。配信の例には、ダウンロード可能なCSVファイル、API、RSSフィードが含まれます。"@ja ;
  rdfs:isDefinedBy <http://www.w3.org/TR/vocab-dcat/> ;
  rdfs:label "Distribuce"@cs ;
  rdfs:label "Distribución"@es ;
  rdfs:label "Distribution"@en ;
  rdfs:label "Distribution"@fr ;
  rdfs:label "Distribuzione"@it ;
  rdfs:label "Διανομή"@el ;
  rdfs:label "التوزيع"@ar ;
  rdfs:label "配信"@ja ;
  skos:scopeNote """Ceci représente une disponibilité générale du jeu de données, et implique qu'il n'existe pas d'information
					sur la méthode d'accès réelle des données, par exple, si c'est un lien de téléchargement direct ou à travers une page Web. """@fr ;
  skos:scopeNote """Esta clase representa una disponibilidad general de un conjunto de datos, e implica que no existe información acerca
          del método de acceso real a los datos, i.e., si es un enlace de descarga directa o a través de una página Web."""@es ;
  skos:scopeNote "Questa classe rappresenta una disponibilità generale di un dataset e non implica alcuna informazione sul metodo di accesso effettivo ai dati, ad esempio se si tratta di un accesso a download diretto, API, o attraverso una pagina Web. L'utilizzo della proprietà dcat:downloadURL indica distribuzioni direttamente scaricabili."@it ;
  skos:scopeNote """This represents a general availability of a dataset it implies no information about the
          actual access method of the data, i.e. whether by direct download, API, or through a Web page.
          The use of dcat:downloadURL property indicates directly downloadable distributions."""@en ;
  skos:scopeNote """Toto popisuje obecnou dostupnost datové sady. Neimplikuje žádnou informaci o skutečné metodě přístupu k datům, tj. zda jsou přímo ke stažení, skrze API či přes webovou stránku. Použití vlastnosti dcat:downloadURL indikuje přímo stažitelné distribuce."""@cs ;
  skos:scopeNote """Αυτό αναπαριστά μία γενική διαθεσιμότητα ενός συνόλου δεδομένων και δεν υπονοεί τίποτα περί του πραγματικού τρόπου πρόσβασης στα δεδομένα, αν είναι άμεσα μεταφορτώσιμα,
					  μέσω API ή μέσω μίας ιστοσελίδας. Η χρήση της ιδιότητας dcat:downloadURL δείχνει μόνο άμεσα μεταφορτώσιμες διανομές."""@el ;
  skos:scopeNote "これは、データセットの一般的な利用可能性を表わし、データの実際のアクセス方式に関する情報（つまり、直接ダウンロードなのか、APIなのか、ウェブページを介したものなのか）を意味しません。dcat:downloadURLプロパティーの使用は、直接ダウンロード可能な配信を意味します。"@ja ;
.
dcat:Relationship
  rdf:type owl:Class ;
  rdfs:comment "An association class for attaching additional information to a relationship between DCAT Resources."@en ;
  rdfs:comment "Una clase de asociación para adjuntar información adicional a una relación entre recursos DCAT."@es ;
  rdfs:comment "Una classe di associazione per il collegamento di informazioni aggiuntive a una relazione tra le risorse DCAT."@it ;
  rdfs:comment "Asociační třída pro připojení dodatečných informací ke vztahu mezi zdroji DCAT."@cs ;
  rdfs:label "Relationship"@en ;
  rdfs:label "Relación"@es ;
  rdfs:label "Relazione"@it ;
  rdfs:label "Vztah"@cs ;
  rdfs:subClassOf [
      rdf:type owl:Restriction ;
      owl:minCardinality "1"^^xsd:nonNegativeInteger ;
      owl:onProperty dct:relation ;
    ] ;
  skos:changeNote "New class added in DCAT 2.0."@en ;
  skos:changeNote "Nueva clase añadida en DCAT 2.0."@es ;
  skos:changeNote "Nuova classe aggiunta in DCAT 2.0."@it ;
  skos:changeNote "Nová třída přidaná ve verzi DCAT 2.0"@cs ;
  skos:scopeNote "Use to characterize a relationship between datasets, and potentially other resources, where the nature of the relationship is known but is not adequately characterized by the standard Dublin Core properties (dct:hasPart, dct:isPartOf, dct:conformsTo, dct:isFormatOf, dct:hasFormat, dct:isVersionOf, dct:hasVersion, dct:replaces, dct:isReplacedBy, dct:references, dct:isReferencedBy, dct:requires, dct:isRequiredBy) or PROV-O properties (prov:wasDerivedFrom, prov:wasInfluencedBy, prov:wasQuotedFrom, prov:wasRevisionOf, prov:hadPrimarySource, prov:alternateOf, prov:specializationOf)"@en ;
  skos:scopeNote "Se usa para caracterizar la relación entre conjuntos de datos, y potencialmente otros recursos, donde la naturaleza de la relación se conoce pero no está caracterizada adecuadamente con propiedades del estándar 'Dublin Core' (dct:hasPart, dct:isPartOf, dct:conformsTo, dct:isFormatOf, dct:hasFormat, dct:isVersionOf, dct:hasVersion, dct:replaces, dct:isReplacedBy, dct:references, dct:isReferencedBy, dct:requires, dct:isRequiredBy) or PROV-O properties (prov:wasDerivedFrom, prov:wasInfluencedBy, prov:wasQuotedFrom, prov:wasRevisionOf, prov:hadPrimarySource, prov:alternateOf, prov:specializationOf)"@es ;
  skos:scopeNote "Viene utilizzato per caratterizzare la relazione tra insiemi di dati, e potenzialmente altri tipi di risorse, nei casi in cui la natura della relazione è nota ma non adeguatamente caratterizzata dalle proprietà dello standard 'Dublin Core' (dct:hasPart, dct:isPartOf, dct:conformsTo, dct:isFormatOf, dct:hasFormat, dct:isVersionOf, dct:hasVersion, dct:replaces, dct:isReplacedBy, dct:references, dct:isReferencedBy, dct:require, dct:isRequiredBy) o dalle propietà fornite da PROV-O  (prov:wasDerivedFrom, prov:wasInfluencedBy, prov:wasQuotedFrom, prov:wasRevisionOf, prov: hadPrimarySource, prov:alternateOf, prov:specializationOf)"@it;
  skos:scopeNote "Používá se pro charakterizaci vztahu mezi datovými sadami a případně i jinými zdroji, kde druh vztahu je sice znám, ale není přiměřeně charakterizován standardními vlastnostmi slovníku Dublin Core (dct:hasPart, dct:isPartOf, dct:conformsTo, dct:isFormatOf, dct:hasFormat, dct:isVersionOf, dct:hasVersion, dct:replaces, dct:isReplacedBy, dct:references, dct:isReferencedBy, dct:requires, dct:isRequiredBy) či vlastnostmi slovníku PROV-O (prov:wasDerivedFrom, prov:wasInfluencedBy, prov:wasQuotedFrom, prov:wasRevisionOf, prov:hadPrimarySource, prov:alternateOf, prov:specializationOf)"@cs ;
.

dcat:Resource
  rdf:type owl:Class ;
  rdfs:comment "Resource published or curated by a single agent."@en ;
  rdfs:comment "Recurso publicado o curado por un agente único."@es ;
  rdfs:comment "Risorsa pubblicata o curata da un singolo agente."@it ;
  rdfs:comment "Zdroj publikovaný či řízený jediným činitelem"@cs ;
  rdfs:label "Catalogued resource"@en ;
  rdfs:label "Recurso catalogado"@es ;
  rdfs:label "Risorsa catalogata"@it ;
  rdfs:label "Katalogizovaný zdroj"@cs ;
  rdfs:subClassOf [
      rdf:type owl:Restriction ;
      owl:minCardinality "1"^^xsd:nonNegativeInteger ;
      owl:onProperty dct:type ;
    ] ;
  skos:changeNote "New class added in DCAT 2.0."@en ;
  skos:changeNote "Nueva clase agregada en DCAT 2.0."@es ;
  skos:changeNote "Nuova classe aggiunta in DCAT 2.0."@it ;
  skos:changeNote "Nová třída přidaná ve verzi DCAT 2.0"@cs ;
  skos:editorialNote "Status: Class accepted by DCAT revision team, but details of definition and constraints not yet resolved."@en ;
  skos:editorialNote "Estado: esta clase se aceptó por el equipo de revisión de DCAT, pero los detalles de la definición y restricciones no están resueltos aún."@es ;
  skos:editorialNote "Stav: Třída přijata týmem pro revizi DCAT, ale detaily definice a omezení ještě nejsou vyřešeny."@cs ;
  skos:scopeNote """The class of all catalogued resources, the Superclass of
    dcat:Dataset, dcat:DataService, dcat:Catalog and any other member of a dcat:Catalog.
    This class carries properties common to all catalogued resources, including datasets and data services.
    It is strongly recommended to use a more specific sub-class. When describing a 
resource which is not a dcat:Dataset or dcat:DataService, it is recommended to create a 
suitable sub-class of dcat:Resource, or use dcat:Resource with the dct:type property to 
indicate the specific type."""@en ;
  skos:scopeNote """La clase de todos los recursos catalogados, la superclase de
        dcat:Dataset, dcat:DataService, dcat:Catalog y cualquier otro miembro de un dcat:Catalog.
        Esta clase tiene propiedades comunes a todos los recursos catalogados, incluyendo conjuntos de datos y servicios de datos.
        Se recomienda fuertemente que se use una clase más específica. Cuando se describe un recurso que no es un dcat:Dataset o dcat:DataService, se recomienda crear una sub-clase apropiada de dcat:Resource, o usar dcat:Resource con la propiedad dct:type to indicar el tipo específico."""@es ;
  skos:scopeNote "La classe di tutte le risorse catalogate, la Superclasse di dcat:Dataset, dcat:DataService, dcat:Catalog e qualsiasi altro membro di dcat:Catalog. Questa classe porta proprietà comuni a tutte le risorse catalogate, inclusi set di dati e servizi dati. Si raccomanda vivamente di utilizzare una sottoclasse più specifica. Quando si descrive una risorsa che non è un dcat:Dataset o dcat:DataService, si raccomanda di creare una sottoclasse di dcat:Resource appropriata, o utilizzare dcat:Resource con la proprietà dct:type per indicare il tipo specifico."@it ;
  skos:scopeNote "Třída všech katalogizovaných zdrojů, nadtřída dcat:Dataset, dcat:DataService, dcat:Catalog a všech ostatních členů dcat:Catalog. Tato třída nese vlastnosti společné všem katalogizovaným zdrojům včetně datových sad a datových služeb. Je silně doporučeno používat specifičtější podtřídy, pokud je to možné. Při popisu zdroje, který není ani dcat:Dataset, ani dcat:DataService se doporučuje vytvořit odpovídající podtřídu dcat:Resrouce a nebo použít dcat:Resource s vlastností dct:type pro určení konkrétního typu."@cs ;
  skos:scopeNote "dcat:Resource is an extension point that enables the definition of any kind of catalog. Additional subclasses may be defined in a DCAT profile or application for catalogs of other kinds of resources."@en ;
  skos:scopeNote "dcat:Resource es un punto de extensión que permite la definición de cualquier tipo de catálogo. Se pueden definir subclases adicionales en perfil de DCAT o una aplicación para catálogos de otro tipo de recursos."@es ;
  skos:scopeNote "dcat:Resource è un punto di estensione che consente la definizione di qualsiasi tipo di catalogo. Sottoclassi aggiuntive possono essere definite in un profilo DCAT o in un'applicazione per cataloghi di altri tipi di risorse."@it ;
  skos:scopeNote "dcat:Resource je bod pro rozšíření umožňující definici různých druhů katalogů. Další podtřídy lze definovat v profilech DCAT či aplikacích pro katalogy zdrojů jiných druhů"@cs ;
  .
dcat:Role
  rdf:type owl:Class ;
  rdfs:label "Role"@en ;
  rdfs:label "Rol"@es ;
  rdfs:label "Ruolo"@it ;
  rdfs:label "Role"@cs ;
  rdfs:seeAlso dcat:hadRole ;
  rdfs:subClassOf skos:Concept ;
  skos:changeNote "New class added in DCAT 2.0."@en ;
  skos:changeNote "Nuova classe aggiunta in DCAT 2.0."@it ;
  skos:changeNote "Nueva clase agregada en DCAT 2.0."@es ;
  skos:changeNote "Nová třída přidaná ve verzi DCAT 2.0"@cs ;
  skos:editorialNote "Introduced into DCAT to complement prov:Role (whose use is limited to roles in the context of an activity, as the range of prov:hadRole)"@en ;
  skos:editorialNote "Incluída en DCAT para complementar prov:Role (cuyo uso está limitado a roles en el contexto de una actividad, ya que es el rango es prov:hadRole)"@es ;
  skos:editorialNote "Introdotta in DCAT per completare prov:Role (il cui uso è limitato ai ruoli nel contesto di un'attività, in conseguenza alla definizione del codominio di prov:hadRole)"@it ;
  skos:editorialNote "Přidáno do DCAT pro doplnění třídy prov:Role (jejíž užití je omezeno na role v kontextu aktivit, jakožto obor hodnot vlastnosti prov:hadRole)"@cs;
  skos:scopeNote "Used in a qualified-attribution to specify the role of an Agent with respect to an Entity. It is recommended that the values be managed as a controlled vocabulary of agent roles, such as http://registry.it.csiro.au/def/isotc211/CI_RoleCode"@en ;
  skos:scopeNote "Se usa en una atribución cualificada para especificar el rol de un Agente con respecto a una Entidad. Se recomienda que los valores se administren como un vocabulario controlado de roles de agente, como por ejemplo http://registry.it.csiro.au/def/isotc211/CI_RoleCode"@es ;
  skos:scopeNote "Utilizzato in un'attribuzione qualificata per specificare il ruolo di un agente rispetto a un'entità. Si consiglia di attribuire i valori considerando un vocabolario controllato dei ruoli dell'agente, ad esempio http://registry.it.csiro.au/def/isotc211/CI_RoleCode"@it ;
  skos:scopeNote "Použito v kvalifikovaném přiřazení pro specifikaci role Agenta ve vztahu k Entitě. Je doporučeno množinu hodnot spravovat jako řízený slovník rolí agentů, jako například http://registry.it.csiro.au/def/isotc211/CI_RoleCode"@cs ;
  skos:scopeNote """Used in a qualified-relation to specify the role of an Entity with respect to another Entity.
  It is recommended that the values be managed as a controlled vocabulary of entity roles such as
  - ISO 19115 DS_AssociationTypeCode http://registry.it.csiro.au/def/isotc211/DS_AssociationTypeCode
  - IANA Registry of Link Relations https://www.iana.org/assignments/link-relation
  - DataCite metadata schema
  - MARC relators https://id.loc.gov/vocabulary/relators"""@en ;
  skos:scopeNote """Se usa en una relación cualificada para especificar el rol de una Entidad con respecto a otra Entidad.
    Se recomienda que los valores se administren como los valores de un vocabulario controlado de roles de entidad como por ejemplo:
    - ISO 19115 DS_AssociationTypeCode http://registry.it.csiro.au/def/isotc211/DS_AssociationTypeCode
    - IANA Registry of Link Relations https://www.iana.org/assignments/link-relation
    - el esquema de metadatos de DataCite
    - MARC relators https://id.loc.gov/vocabulary/relators"""@es ;
  skos:scopeNote "Utilizzato in una relazione qualificata per specificare il ruolo di un'entità rispetto a un'altra entità. Si raccomanda che il valore sia preso da un vocabolario controllato di ruoli di entità come ISO 19115 DS_AssociationTypeCode http://registry.it.csiro.au/def/isotc211/DS_AssociationTypeCode, IANA Registry of Link Relations https://www.iana.org/assignments/link-relation, DataCite metadata schema, o MARC relators https://id.loc.gov/vocabulary/relators"@it ;
  skos:scopeNote "Použito v kvalifikovaném vztahu pro specifikaci role Entity ve vztahu k jiné Entitě. Je doporučeno množinu hodnot spravovat jako řízený slovník rolí entit, jako například ISO 19115 DS_AssociationTypeCode http://registry.it.csiro.au/def/isotc211/DS_AssociationTypeCode, IANA Registry of Link Relations https://www.iana.org/assignments/link-relation, DataCite metadata schema, či MARC relators https://id.loc.gov/vocabulary/relators"@cs ;
  rdfs:comment "A role is the function of a resource or agent with respect to another resource, in the context of resource attribution or resource relationships."@en ;
  rdfs:comment "Un rol es la función de un recurso o agente con respecto a otro recuros, en el contexto de atribución del recurso o de las relaciones entre recursos."@es ;
  rdfs:comment "Un ruolo è la funzione di una risorsa o di un agente rispetto ad un'altra risorsa, nel contesto dell'attribuzione delle risorse o delle relazioni tra risorse."@it ;
  rdfs:comment "Role je funkce zdroje či agenta ve vztahu k jinému zdroji, v kontextu přiřazení zdrojů či vztahů mezi zdroji."@en ;
.
dcat:accessService
  rdf:type owl:ObjectProperty ;
  rdfs:comment "A site or end-point that gives access to the distribution of the dataset."@en ;
  rdfs:comment "Un sito o end-point che dà accesso alla distribuzione del set di dati."@it ;
  rdfs:comment "Un sitio o end-point que da acceso a la distribución de un conjunto de datos."@es ;
  rdfs:comment "Umístění či přístupový bod zpřístupňující distribuci datové sady"@cs ;  
  rdfs:label "data access service"@en ;
  rdfs:label "servizio di accesso ai dati"@it ;
  rdfs:label "servicio de acceso de datos"@es ;
  rdfs:label "služba pro přístup k datům"@cs ;
  rdfs:range dcat:DataService ;
  skos:changeNote "New property added in DCAT 2.0."@en ;
  skos:changeNote "Nueva propiedad agregada en DCAT 2.0."@es ;
  skos:changeNote "Nuova proprietà aggiunta in DCAT 2.0."@it ;
  skos:changeNote "Nová vlastnost přidaná ve verzi DCAT 2.0"@cs ;
.
dcat:accessURL
  rdf:type rdf:Property ;
  rdf:type owl:ObjectProperty ;
  rdfs:comment """A URL of a resource that gives access to a distribution of the dataset. E.g. landing page, feed, SPARQL endpoint.
          Use for all cases except a simple download link, in which case downloadURL is preferred."""@en ;
  rdfs:comment """Ceci peut être tout type d'URL qui donne accès à une distribution du jeu de données. Par exemple, un lien à une page HTML contenant un lien au jeu de données,
					un Flux RSS, un point d'accès SPARQL. Utilisez le lorsque votre catalogue ne contient pas d'information sur quoi il est ou quand ce n'est pas téléchargeable."""@fr ;
  rdfs:comment "Un URL di una risorsa che consente di accedere a una distribuzione del set di dati. Per esempio, pagina di destinazione, feed, endpoint SPARQL. Da utilizzare per tutti i casi, tranne  quando  si tratta di un semplice link per il download nel qual caso è preferito downloadURL."@it ;
  rdfs:comment """Puede ser cualquier tipo de URL que de acceso a una distribución del conjunto de datos, e.g., página de destino, descarga,
					URL feed, punto de acceso SPARQL. Esta propriedad se debe usar cuando su catálogo de datos no tiene información sobre donde está o cuando no se puede descargar."""@es ;
  rdfs:comment "URL zdroje, přes které je přístupná distribuce datové sady. Příkladem může být vstupní stránka, RSS kanál či SPARQL endpoint. Použijte ve všech případech kromě URL souboru ke stažení, pro které je lepší použít dcat:downloadURL."@cs ;
  rdfs:comment """Μπορεί να είναι οποιουδήποτε είδους URL που δίνει πρόσβαση στη διανομή ενός συνόλου δεδομένων. Π.χ. ιστοσελίδα αρχικής πρόσβασης,
          μεταφόρτωση, feed URL, σημείο διάθεσης SPARQL. Να χρησιμοποιείται όταν ο κατάλογος δεν περιέχει πληροφορίες εαν πρόκειται ή όχι για μεταφορτώσιμο αρχείο."""@el ;
  rdfs:comment "أي رابط يتيح الوصول إلى البيانات. إذا كان الرابط هو ربط مباشر لملف يمكن تحميله استخدم الخاصية downloadURL"@ar ;
  rdfs:comment "データセットの配信にアクセス権を与えるランディング・ページ、フィード、SPARQLエンドポイント、その他の種類の資源。"@ja ;
  rdfs:domain dcat:Distribution ;
  rdfs:isDefinedBy <http://www.w3.org/TR/vocab-dcat/> ;
  rdfs:label "URL d'accès"@fr ;
  rdfs:label "URL de acceso"@es ;
  rdfs:label "indirizzo di accesso"@it ;
  rdfs:label "URL πρόσβασης"@el ;
  rdfs:label "access address"@en ;
  rdfs:label "přístupová adresa"@cs ;
  rdfs:label "رابط وصول"@ar ;
  rdfs:label "アクセスURL"@ja ;
  rdfs:range rdfs:Resource ;
  owl:propertyChainAxiom (
      dcat:accessService
      dcat:endpointURL
    ) ;
  skos:editorialNote "Status: English Definition text modified by DCAT revision team, updated Italian and Czech translation provided, translations for other languages pending."@en ;
  skos:editorialNote "rdfs:label, rdfs:comment and skos:scopeNote have been modified. Non-english versions except for Italian must be updated."@en ;
  skos:scopeNote """El rango es una URL.
          Si la distribución es accesible solamente través de una página de destino (es decir, si no se conoce una URL de descarga directa),
          entonces el enlance a la página de destino debe ser duplicado como accessURL en la distribución."""@es ;
  skos:scopeNote "Pokud jsou distribuce přístupné pouze přes vstupní stránku (tj. URL pro přímé stažení nejsou známa), pak by URL přístupové stránky mělo být duplikováno ve vlastnosti distribuce accessURL."@cs ;
  skos:scopeNote """If the distribution(s) are accessible only through a landing page (i.e. direct download URLs are not known),
          then the landing page link should be duplicated as accessURL on a distribution."""@en ;
  skos:scopeNote "Se le distribuzioni sono accessibili solo attraverso una pagina web (ad esempio, gli URL per il download diretto non sono noti), allora il link della pagina web deve essere duplicato come accessURL sulla distribuzione."@it ;
  skos:scopeNote """La valeur est une URL.
						Si la distribution est accessible seulement au travers d'une page d'atterrissage (c-à-dire on n'ignore une URL de téléchargement direct) ,
						alors le lien à la page d'atterrissage doit être dupliqué comee accessURL sur la distribution."""@fr ;
  skos:scopeNote """Η τιμή είναι ένα URL.
					Αν η/οι διανομή/ές είναι προσβάσιμη/ες μόνο μέσω μίας ιστοσελίδας αρχικής πρόσβασης (δηλαδή αν δεν υπάρχουν γνωστές διευθύνσεις άμεσης μεταφόρτωσης), τότε ο σύνδεσμος της ιστοσελίδας αρχικής πρόσβασης πρέπει να αναπαραχθεί ως accessURL σε μία διανομή."""@el ;
  skos:scopeNote """確実にダウンロードでない場合や、ダウンロードかどうかが不明である場合は、downloadURLではなく、accessURLを用いてください。
ランディング・ページを通じてしか配信にアクセスできない場合（つまり、直接的なダウンロードURLが不明）は、配信におけるaccessURLとしてランディング・ページのリンクをコピーすべきです（SHOULD）。"""@ja ;
.
dcat:bbox
  rdfs:label "bounding box"@en;
  rdfs:label "cuadro delimitador"@es;
  rdfs:label "ohraničení oblasti"@cs;
  rdf:type rdf:Property ;
  rdf:type owl:DatatypeProperty ;
  rdfs:domain dct:Location ;
  rdfs:range rdfs:Literal ;
  skos:definition "The geographic bounding box of a resource"@en ;
  skos:definition "El cuadro delimitador geográfico para un recurso."@es ;
  skos:definition "Ohraničení geografické oblasti zdroje"@cs ;
  skos:changeNote "New property added in DCAT 2.0."@en ;
  skos:changeNote "Propiedad nueva agregada en DCAT 2.0."@es ;
  skos:changeNote "Nová vlastnost přidaná ve verzi DCAT 2.0"@cs ;
  skos:scopeNote "The range of this property is intentionally generic, with the purpose of allowing different geometry encodings. E.g., the geometry could be encoded with as WKT (geosparql:asWKT [GeoSPARQL]) or [GML] (geosparql:asGML [GeoSPARQL])."@en ;
  skos:scopeNote "El rango de esta propiedad es intencionalmente genérico con el propósito de permitir distintas codificaciones geométricas. Por ejemplo, la geometría puede ser codificada como WKT (geosparql:asWKT [GeoSPARQL]) o [GML] (geosparql:asGML [GeoSPARQL])."@es ;
  skos:scopeNote "Obor hodnot této vlastnosti je úmyslně obecný, aby umožnil různé kódování geometrií. Geometrie by kupříkladu mohla být kódována jako WKT (geosparql:asWKT [GeoSPARQL]) či [GML] (geosparql:asGML [GeoSPARQL])."@cs ;
.
dcat:byteSize
  rdf:type rdf:Property ;
  rdf:type owl:DatatypeProperty ;
  rdfs:comment "El tamaño de una distribución en bytes"@es ;
  rdfs:comment "La dimensione di una distribuzione in byte."@it ;
  rdfs:comment "La taille de la distribution en octects"@fr ;
  rdfs:comment "The size of a distribution in bytes."@en ;
  rdfs:comment "Velikost distribuce v bajtech."@cs ;
  rdfs:comment "Το μέγεθος μιας διανομής σε bytes."@el ;
  rdfs:comment "الحجم بالبايتات "@ar ;
  rdfs:comment "バイトによる配信のサイズ。"@ja ;
  rdfs:domain dcat:Distribution ;
  rdfs:isDefinedBy <http://www.w3.org/TR/vocab-dcat/> ;
  rdfs:label "byte size"@en ;
  rdfs:label "dimensione in byte"@it ;
  rdfs:label "taille en octects"@fr ;
  rdfs:label "tamaño en bytes"@es ;
  rdfs:label "velikost v bajtech"@cs ;
  rdfs:label "μέγεθος σε bytes"@el ;
  rdfs:label "الحجم بالبايت"@ar ;
  rdfs:label "バイト・サイズ"@ja ;
  rdfs:range rdfs:Literal ;
  skos:scopeNote """El tamaño en bytes puede ser aproximado cuando se desconoce el tamaño exacto.
          El valor literal de dcat:byteSize debe tener tipo 'xsd:decimal'"""@es ;
  skos:scopeNote "La dimensione in byte può essere approssimata quando non si conosce la dimensione precisa. Il valore di dcat:byteSize dovrebbe essere espresso come un xsd:decimal"@it ;
  skos:scopeNote """La taille en octects peut être approximative lorsque l'on ignore la taille réelle.
					La valeur littérale de dcat:byteSize doit être de type xsd:decimal"""@fr ;
  skos:scopeNote """The size in bytes can be approximated when the precise size is not known.
          The literal value of dcat:byteSize should by typed as xsd:decimal"""@en ;
  skos:scopeNote "Velikost v bajtech může být přibližná, pokud její přesná hodnota není známa. Literál s hodnotou dcat:byteSize by měl mít datový typ xsd:decimal"@cs ;
  skos:scopeNote """Το μέγεθος σε bytes μπορεί να προσεγγιστεί όταν η ακριβής τιμή δεν είναι γνωστή.
          Η τιμή της dcat:byteSize θα πρέπει να δίνεται με τύπο δεδομένων xsd:decimal"""@el ;
  skos:scopeNote "الحجم يمكن أن يكون تقريبي إذا كان الحجم الدقيق غير معروف"@ar ;
  skos:scopeNote "正確なサイズが不明である場合、サイズは、バイトによる近似値を示すことができます。"@ja ;
.
dcat:catalog
  rdf:type owl:ObjectProperty ;
  rdfs:comment "A catalog whose contents are of interest in the context of this catalog."@en ;
  rdfs:comment "Un catálogo cuyo contenido es de interés en el contexto del catálogo que está siendo descripto."@es ;
  rdfs:comment "Un catalogo i cui contenuti sono di interesse nel contesto di questo catalogo."@it ;
  rdfs:comment "Katalog, jehož obsah je v kontextu tohoto katalogu zajímavý"@cs ;
  rdfs:domain dcat:Catalog ;
  rdfs:label "catalog"@en ;
  rdfs:label "catalogo"@it ;
  rdfs:label "catálogo"@es ;
  rdfs:label "katalog"@cs ;
  rdfs:range dcat:Catalog ;
  rdfs:subPropertyOf dct:hasPart ;
  rdfs:subPropertyOf rdfs:member ;
  skos:changeNote "New property added in DCAT 2.0."@en ;
  skos:changeNote "Nueva propiedad agregada en DCAT 2.0."@es ;
  skos:changeNote "Nuova proprietà aggiunta in DCAT 2.0."@it ;
  skos:changeNote "Nová vlastnost přidaná ve verzi DCAT 2.0"@cs ;
.
dcat:centroid
  rdfs:label "centroid"@en;
  rdfs:label "centroide"@es;
  rdfs:label "centroid"@cs;
  rdf:type rdf:Property ;
  rdf:type owl:DatatypeProperty ;
  rdfs:domain dct:Location ;
  rdfs:range rdfs:Literal ;
  skos:definition "The geographic center (centroid) of a resource."@en ;
  skos:definition "El centro geográfico (centroide) de un recurso."@es ;
  skos:definition "Geografický střed (centroid) zdroje"@cs ;
  skos:changeNote "New property added in DCAT 2.0."@en ;
  skos:changeNote "Nueva propiedad agregada en DCAT 2.0."@es ;
  skos:changeNote "Nová vlastnost přidaná ve verzi DCAT 2.0"@cs ;
  skos:scopeNote "The range of this property is intentionally generic, with the purpose of allowing different geometry encodings. E.g., the geometry could be encoded with as WKT (geosparql:asWKT [GeoSPARQL]) or [GML] (geosparql:asGML [GeoSPARQL])."@en ;
  skos:scopeNote "El rango de esta propiedad es intencionalmente genérico con el objetivo de permitir distintas codificaciones geométricas. Por ejemplo, la geometría puede codificarse como WKT (geosparql:asWKT [GeoSPARQL]) o [GML] (geosparql:asGML [GeoSPARQL])."@es ;
  skos:scopeNote "Obor hodnot této vlastnosti je úmyslně obecný, aby umožnil různé kódování geometrií. Geometrie by kupříkladu mohla být kódována jako WKT (geosparql:asWKT [GeoSPARQL]) či [GML] (geosparql:asGML [GeoSPARQL])."@cs ;
.
dcat:contactPoint
  rdf:type rdf:Property ;
  rdf:type owl:ObjectProperty ;
  rdfs:comment "Informazioni di contatto rilevanti per la risorsa catalogata. Si raccomanda l'uso di vCard."@it ;
  rdfs:comment "Relevantní kontaktní informace pro katalogizovaný zdroj. Doporučuje se použít slovník VCard."@cs ;
  rdfs:comment "Información relevante de contacto para el recurso catalogado. Se recomienda el uso de vCard."@es ;
  rdfs:comment "Relevant contact information for the catalogued resource. Use of vCard is recommended."@en ;
  rdfs:comment "Relie un jeu de données à une information de contact utile en utilisant VCard."@fr ;
  rdfs:comment "Συνδέει ένα σύνολο δεδομένων με ένα σχετικό σημείο επικοινωνίας, μέσω VCard."@el ;
  rdfs:comment "تربط قائمة البيانات بعنوان اتصال موصف  باستخدام VCard"@ar ;
  rdfs:comment "データセットを、VCardを用いて提供されている適切な連絡先情報にリンクします。"@ja ;
  rdfs:isDefinedBy <http://www.w3.org/TR/vocab-dcat/> ;
  rdfs:label "Punto de contacto"@es ;
  rdfs:label "contact point"@en ;
  rdfs:label "kontaktní bod"@cs ;
  rdfs:label "point de contact"@fr ;
  rdfs:label "punto di contatto"@it ;
  rdfs:label "σημείο επικοινωνίας"@el ;
  rdfs:label "عنوان اتصال"@ar ;
  rdfs:label "窓口"@ja ;
  rdfs:range vcard:Kind ;
  skos:editorialNote "Status: English Definition text modified by DCAT revision team, Italian, Spanish and Czech translations provided, other translations pending."@en ;
.
dcat:dataset
  rdf:type rdf:Property ;
  rdf:type owl:ObjectProperty ;
  rdfs:comment "A collection of data that is listed in the catalog."@en ;
  rdfs:comment "Una raccolta di dati che è elencata nel catalogo."@it ;
  rdfs:comment "Un conjunto de datos que se lista en el catálogo"@es ;
  rdfs:comment "Kolekce dat, která je katalogizována v katalogu."@cs ;
  rdfs:comment "Relie un catalogue à un jeu de données faisant partie de ce catalogue"@fr ;
  rdfs:comment "Συνδέει έναν κατάλογο με ένα σύνολο δεδομένων το οποίο ανήκει στον εν λόγω κατάλογο."@el ;
  rdfs:comment "تربط الفهرس بقائمة بيانات ضمنه"@ar ;
  rdfs:comment "カタログの一部であるデータセット。"@ja ;
  rdfs:domain dcat:Catalog ;
  rdfs:isDefinedBy <http://www.w3.org/TR/vocab-dcat/> ;
  rdfs:label "conjunto de datos"@es ;
  rdfs:label "dataset"@en ;
  rdfs:label "dataset"@it ;
  rdfs:label "datová sada"@cs ;
  rdfs:label "jeu de données"@fr ;
  rdfs:label "σύνολο δεδομένων"@el ;
  rdfs:label "قائمة بيانات"@ar ;
  rdfs:label "データセット"@ja ;
  rdfs:range dcat:Dataset ;
  rdfs:subPropertyOf dct:hasPart ;
  rdfs:subPropertyOf rdfs:member ;
  skos:editorialNote "Status: English Definition text modified by DCAT revision team, Italian, Spanish and Czech translation provided, other translations pending."@en ;
.
dcat:distribution
  rdf:type rdf:Property ;
  rdf:type owl:ObjectProperty ;
  rdfs:comment "An available distribution of the dataset."@en ;
  rdfs:comment "Una distribuzione disponibile per il set di dati."@it ;
  rdfs:comment "Una distribución disponible del conjunto de datos."@es ;
  rdfs:comment "Connecte un jeu de données à des distributions disponibles."@fr ;
  rdfs:comment "Dostupná distribuce datové sady."@cs ;
  rdfs:comment "Συνδέει ένα σύνολο δεδομένων με μία από τις διαθέσιμες διανομές του."@el ;
  rdfs:comment "تربط قائمة البيانات بطريقة أو بشكل يسمح  الوصول الى البيانات"@ar ;
  rdfs:comment "データセットを、その利用可能な配信に接続します。"@ja ;
  rdfs:domain dcat:Dataset ;
  rdfs:isDefinedBy <http://www.w3.org/TR/vocab-dcat/> ;
  rdfs:label "distribuce"@cs ;
  rdfs:label "distribución"@es ;
  rdfs:label "distribution"@en ;
  rdfs:label "distribution"@fr ;
  rdfs:label "distribuzione"@it ;
  rdfs:label "διανομή"@el ;
  rdfs:label "توزيع"@ar ;
  rdfs:label "データセット配信"@ja ;
  rdfs:range dcat:Distribution ;
  rdfs:subPropertyOf dct:relation ;
  skos:editorialNote "Status: English Definition text modified by DCAT revision team, translations pending (except for Italian, Spanish and Czech)."@en ;
.
dcat:downloadURL
  rdf:type rdf:Property ;
  rdf:type owl:ObjectProperty ;
  rdfs:comment """The URL of the downloadable file in a given format. E.g. CSV file or RDF file. The
            format is indicated by the distribution's dct:format and/or dcat:mediaType"""@en ;
  rdfs:comment """La URL de un archivo descargable en el formato dato. Por ejemplo, archivo CSV o archivo RDF. El
            formato se describe con las propiedades de la distribución dct:format y/o dcat:mediaType"""@es ;
  rdfs:comment """Ceci est un lien direct à un fichier téléchargeable en un format donnée. Exple fichier CSV ou RDF. Le format
					est décrit par les propriétés de distribution dct:format et/ou dcat:mediaType"""@fr ;
  rdfs:comment "Questo è un link diretto al file scaricabile in un dato formato. E.g. un file CSV o un file RDF. Il formato è descritto dal dct:format e/o dal dcat:mediaType della distribuzione."@it ;
  rdfs:comment "URL souboru ke stažení v daném formátu, například CSV nebo RDF soubor. Formát je popsán vlastností distribuce dct:format a/nebo dcat:mediaType."@cs ;
  rdfs:comment "dcat:downloadURLはdcat:accessURLの特定の形式です。しかし、DCATプロファイルが非ダウンロード・ロケーションに対してのみaccessURLを用いる場合には、より強い分離を課すことを望む可能性があるため、この含意を強化しないように、DCATは、dcat:downloadURLをdcat:accessURLのサブプロパティーであると定義しません。"@ja ;
  rdfs:comment """Είναι ένας σύνδεσμος άμεσης μεταφόρτωσης ενός αρχείου σε μια δεδομένη μορφή. Π.χ. ένα αρχείο CSV ή RDF.
					Η μορφη αρχείου περιγράφεται από τις ιδιότητες dct:format ή/και dcat:mediaType της διανομής"""@el ;
  rdfs:comment "رابط مباشر لملف يمكن تحميله. نوع الملف يتم توصيفه باستخدام الخاصية dct:format dcat:mediaType "@ar ;
  rdfs:domain dcat:Distribution ;
  rdfs:isDefinedBy <http://www.w3.org/TR/vocab-dcat/> ;
  rdfs:label "URL de descarga"@es ;
  rdfs:label "URL de téléchargement"@fr ;
  rdfs:label "URL di scarico"@it ;
  rdfs:label "URL souboru ke stažení"@cs ;
  rdfs:label "URL μεταφόρτωσης"@el ;
  rdfs:label "download URL"@en ;
  rdfs:label "رابط تحميل"@ar ;
  rdfs:label "ダウンロードURL"@ja ;
  rdfs:range rdfs:Resource ;
  skos:editorialNote "Status: English  Definition text modified by DCAT revision team, Italian, Spanish and Czech translation updated, other translations pending."@en ;
  skos:editorialNote "rdfs:label, rdfs:comment and/or skos:scopeNote have been modified. Non-english versions must be updated."@en ;
  skos:scopeNote "El valor es una URL."@es ;
  skos:scopeNote "dcat:downloadURL BY MĚLA být použita pro adresu, ze které je distribuce přímo přístupná, typicky skrze požadavek HTTP Get."@cs ;
  skos:scopeNote "dcat:downloadURL DOVREBBE essere utilizzato per l'indirizzo a cui questa distribuzione è disponibile direttamente, in genere attraverso una richiesta Get HTTP."@it ;
  skos:scopeNote "La valeur est une URL."@fr ;
  skos:scopeNote "dcat:downloadURL SHOULD be used for the address at which this distribution is available directly, typically through a HTTP Get request."@en ;
  skos:scopeNote "Η τιμή είναι ένα URL."@el ;
.
dcat:endDate
  rdfs:label "end date"@en;
  rdfs:label "fecha final"@es;
  rdfs:label "datum konce"@cs;
  rdf:type rdf:Property ;
  rdf:type owl:DatatypeProperty ;
  rdfs:domain dct:PeriodOfTime ;
  rdfs:range rdfs:Literal ;
  skos:definition "The end of the period"@en ;
  skos:definition "El fin del período."@es ;
  skos:definition "Konec doby trvání"@cs ;
  skos:changeNote "New property added in DCAT 2.0."@en ;
  skos:changeNote "Nueva propiedad agregada en DCAT 2.0."@es ;
  skos:changeNote "Nová vlastnost přidaná ve verzi DCAT 2.0"@cs ;
  skos:scopeNote "The range of this property is intentionally generic, with the purpose of allowing different level of temporal precision for specifying the end of a period. E.g., it can be expressed with a date (xsd:date), a date and time (xsd:dateTime), or a year (xsd:gYear)."@en ;
  skos:scopeNote "El rango de esta propiedad es intencionalmente genérico con el propósito de permitir distintos niveles de precisión temporal para especificar el fin del período. Por ejemplo, puede expresarse como una fecha (xsd:date), una fecha y un tiempo (xsd:dateTime), o un año (xsd:gYear)."@es ;
  skos:scopeNote "Obor hodnot této vlastnosti je úmyslně obecný, aby umožnil různé úrovně časového rozlišení pro specifikaci konce doby trvání. Ten může být kupříkladu vyjádřen datumem (xsd:date), datumem a časem (xsd:dateTime) či rokem (xsd:gYear)."@cs ;
.
dcat:endpointDescription
  rdf:type owl:ObjectProperty ;
  rdfs:comment "A description of the service end-point, including its operations, parameters etc."@en ;
  rdfs:comment "Una descrizione dell'endpoint del servizio, incluse le sue operazioni, parametri, ecc."@it ;
  rdfs:comment "Una descripción del end-point del servicio, incluyendo sus operaciones, parámetros, etc.."@es ;
  rdfs:comment "Popis přístupového bodu služby včetně operací, parametrů apod."@cs ;
  rdfs:domain dcat:DataService ;
  rdfs:label "description of service end-point"@en ;
  rdfs:label "descrizione dell'endpoint del servizio"@it ;
  rdfs:label "descripción del end-point del servicio"@es ;
  rdfs:label "popis přístupového bodu služby"@cs ;
  skos:changeNote "New property in DCAT 2.0."@en ;
  skos:changeNote "Nuova proprietà in DCAT 2.0."@it ;
  skos:changeNote "Nueva propiedad agregada en DCAT 2.0."@en ;
  skos:changeNote "Nová vlastnost přidaná ve verzi DCAT 2.0"@cs ;
  skos:scopeNote "An endpoint description may be expressed in a machine-readable form, such as an OpenAPI (Swagger) description, an OGC GetCapabilities response, a SPARQL Service Description, an OpenSearch or WSDL document, a Hydra API description, else in text or some other informal mode if a formal representation is not possible."@en ;
  skos:scopeNote "Una descrizione dell'endpoint può essere espressa in un formato leggibile dalla macchina, come una descrizione OpenAPI (Swagger), una risposta GetCapabilities OGC, una descrizione del servizio SPARQL, un documento OpenSearch o WSDL, una descrizione API Hydra, o con del testo o qualche altra modalità informale se una rappresentazione formale non è possibile."@it ;
  skos:scopeNote "Una descripción del endpoint del servicio puede expresarse en un formato que la máquina puede interpretar, tal como una descripción basada en OpenAPI (Swagger), una respuesta OGC GetCapabilities, una descripción de un servicio SPARQL, un documento OpenSearch o WSDL, una descripción con la Hydra API, o en texto u otro modo informal si la representación formal no es posible."@es ;
  skos:scopeNote "Popis přístupového bodu může být vyjádřen ve strojově čitelné formě, například jako popis OpenAPI (Swagger), odpověď služby OGC getCapabilities, pomocí slovníku SPARQL Service Description, jako OpenSearch či WSDL document, jako popis API dle slovníku Hydra, a nebo textově nebo jiným neformálním způsobem, pokud není možno použít formální reprezentaci."@cs ;
  skos:scopeNote "The endpoint decription gives specific details of the actual endpoint instance, while dct:conformsTo is used to indicate the general standard or specification that the endpoint implements."@en ;
  skos:scopeNote "La descrizione dell'endpoint fornisce dettagli specifici dell'istanza dell'endpoint reale, mentre dct:conformsTo viene utilizzato per indicare lo standard o le specifiche implementate dall'endpoint."@it ;
  skos:scopeNote "La descripción del endpoint brinda detalles específicos de la instancia del endpoint, mientras que dct:conformsTo se usa para indicar el estándar general o especificación que implementa el endpoint."@es ;
  skos:scopeNote "Popis přístupového bodu dává specifické detaily jeho konkrétní instance, zatímco dct:conformsTo indikuje obecný standard či specifikaci kterou přístupový bod implementuje."@cs ;
.
dcat:endpointURL
  rdf:type owl:ObjectProperty ;
  rdfs:comment "The root location or primary endpoint of the service (a web-resolvable IRI)"@en ;
  rdfs:comment "La locazione principale o l'endpoint primario del servizio (un IRI risolvibile via web)"@it;
  rdfs:comment "La posición raíz o end-point principal del servicio (una IRI web) "@es;
  rdfs:comment "Kořenové umístění nebo hlavní přístupový bod služby (IRI přístupné přes Web)"@cs ;
  rdfs:domain dcat:DataService ;
  rdfs:range rdfs:Resource ;
  rdfs:label "service end-point"@en ;
  rdfs:label "end-point del servizio"@it ;
  rdfs:label "end-point del servicio"@es ;
  rdfs:label "přístupový bod služby"@cs ;
  skos:changeNote "New property in DCAT 2.0."@en ;
  skos:changeNote "Nuova proprietà in DCAT 2.0."@it ;
  skos:changeNote "Nueva propiedad agregada en DCAT 2.0."@es ;
  skos:changeNote "Nová vlastnost přidaná ve verzi DCAT 2.0"@cs ;
.
dcat:hadRole
  rdf:type owl:ObjectProperty ;
  rdfs:comment "The function of an entity or agent with respect to another entity or resource."@en ;
  rdfs:comment "La función de una entidad o agente con respecto a otra entidad o recurso."@es ;
  rdfs:comment "La funzione di un'entità o un agente rispetto ad un'altra entità o risorsa."@it ;
  rdfs:comment "Funkce entity či agenta ve vztahu k jiné entitě či zdroji."@cs ;
  rdfs:domain [
      rdf:type owl:Class ;
      owl:unionOf (
          prov:Attribution
          dcat:Relationship
        ) ;
    ] ;
  rdfs:label "hadRole"@en ;
  rdfs:label "haRuolo"@it ;
  rdfs:label "tiene rol"@it ;
  rdfs:label "sehraná role"@cs ;
  rdfs:range dcat:Role ;
  skos:changeNote "New property added in DCAT 2.0."@en ;
  skos:changeNote "Nuova proprietà aggiunta in DCAT 2.0."@it ;
  skos:changeNote "Nueva propiedad agregada en DCAT 2.0."@es ;
  skos:changeNote "Nová vlastnost přidaná ve verzi DCAT 2.0"@cs ;
  skos:editorialNote "Introduced into DCAT to complement prov:hadRole (whose use is limited to roles in the context of an activity, with the domain of prov:Association"@en ;
  skos:editorialNote "Introdotta in DCAT per completare prov:hadRole (il cui uso è limitato ai ruoli nel contesto di un'attività, con il dominio di prov:Association."@it ;
  skos:editorialNote "Agregada en DCAT para complementar prov:hadRole (cuyo uso está limitado a roles en el contexto de una actividad, con dominio prov:Association."@es ;
  skos:editorialNote "Přidáno do DCAT pro doplnění vlastnosti prov:hadRole (jejíž užití je omezeno na role v kontextu aktivity, s definičním oborem prov:Association)"@cs ;
  skos:scopeNote "May be used in a qualified-attribution to specify the role of an Agent with respect to an Entity. It is recommended that the value be taken from a controlled vocabulary of agent roles, such as http://registry.it.csiro.au/def/isotc211/CI_RoleCode"@en ;
  skos:scopeNote "Puede usarse en una atribución cualificada para especificar el rol de un Agente con respecto a una Entidad. Se recomienda que el valor sea de un vocabulario controlado de roles de agentes, como por ejemplo http://registry.it.csiro.au/def/isotc211/CI_RoleCode"@es ;
  skos:scopeNote "Può essere utilizzato in un'attribuzione qualificata per specificare il ruolo di un agente rispetto a un'entità. Si raccomanda che il valore sia preso da un vocabolario controllato di ruoli di agente, come ad esempio http://registry.it.csiro.au/def/isotc211/CI_RoleCode"@it ;
  skos:scopeNote "Může být použito v kvalifikovaném přiřazení pro specifikaci role Agenta ve vztahu k Entitě. Je doporučeno hodnotu vybrat z řízeného slovníku rolí agentů, jako například http://registry.it.csiro.au/def/isotc211/CI_RoleCode"@cs ;
  skos:scopeNote """May be used in a qualified-relation to specify the role of an Entity with respect to another Entity.
  It is recommended that the value be taken from a controlled vocabulary of entity roles such as
  - ISO 19115 DS_AssociationTypeCode http://registry.it.csiro.au/def/isotc211/DS_AssociationTypeCode
  - IANA Registry of Link Relations https://www.iana.org/assignments/link-relation
  - DataCite metadata schema
  - MARC relators https://id.loc.gov/vocabulary/relators"""@en ;
  skos:scopeNote """Puede usarse en una atribución cualificada para especificar el rol de una Entidad con respecto a otra Entidad.
  Se recomienda que su valor se tome de un vocabulario controlado de roles de entidades como por ejemplo:
  - ISO 19115 DS_AssociationTypeCode http://registry.it.csiro.au/def/isotc211/DS_AssociationTypeCode
  - IANA Registry of Link Relations https://www.iana.org/assignments/link-relation
  - esquema de metadatos de DataCite
  - MARC relators https://id.loc.gov/vocabulary/relators"""@es ;
  skos:scopeNote "Può essere utilizzata in una relazione qualificata per specificare il ruolo di un'entità rispetto a un'altra entità. Si raccomanda che il valore sia preso da un vocabolario controllato di ruoli di entità come ISO 19115 DS_AssociationTypeCode http://registry.it.csiro.au/def/isotc211/DS_AssociationTypeCode, IANA Registry of Link Relations https://www.iana.org/assignments/link-relation, DataCite metadata schema, o MARC relators https://id.loc.gov/vocabulary/relators"@it ;
  skos:scopeNote "Může být použito v kvalifikovaném vztahu pro specifikaci role Entity ve vztahu k jiné Entitě. Je doporučeno použít hodnotu z řízeného slovníku rolí entit, jako například ISO 19115 DS_AssociationTypeCode http://registry.it.csiro.au/def/isotc211/DS_AssociationTypeCode, IANA Registry of Link Relations https://www.iana.org/assignments/link-relation, DataCite metadata schema, MARC relators https://id.loc.gov/vocabulary/relators"@cs ;
.
dcat:keyword
  rdf:type rdf:Property ;
  rdf:type owl:DatatypeProperty ;
  rdfs:comment "A keyword or tag describing a resource."@en ;
  rdfs:comment "Klíčové slovo nebo značka popisující zdroj."@cs ;
  rdfs:comment "Un mot-clé ou étiquette décrivant une ressource."@fr ;
  rdfs:comment "Una palabra clave o etiqueta que describe un recurso."@es ;
  rdfs:comment "Una parola chiave o un'etichetta per descrivere la risorsa."@it ;
  rdfs:comment "Μία λέξη-κλειδί ή μία ετικέτα που περιγράφει το σύνολο δεδομένων."@el ;
  rdfs:comment "كلمة  مفتاحيه توصف قائمة البيانات"@ar ;
  rdfs:comment "データセットを記述しているキーワードまたはタグ。"@ja ;
  rdfs:isDefinedBy <http://www.w3.org/TR/vocab-dcat/> ;
  rdfs:label "keyword"@en ;
  rdfs:label "klíčové slovo"@cs ;
  rdfs:label "mot-clés "@fr ;
  rdfs:label "palabra clave"@es ;
  rdfs:label "parola chiave"@it ;
  rdfs:label "λέξη-κλειδί"@el ;
  rdfs:label "كلمة  مفتاحية "@ar ;
  rdfs:label "キーワード/タグ"@ja ;
  rdfs:range rdfs:Literal ;
  rdfs:subPropertyOf dct:subject ;
.
dcat:landingPage
  rdf:type rdf:Property ;
  rdf:type owl:ObjectProperty ;
  rdfs:comment "A Web page that can be navigated to in a Web browser to gain access to the catalog, a dataset, its distributions and/or additional information."@en ;
  rdfs:comment "Una pagina web che può essere navigata per ottenere l'accesso al catalogo, ad un dataset, alle distribuzioni del dataset e/o ad informazioni addizionali."@it ;
  rdfs:comment "Una página web que puede ser visitada en un explorador Web para tener acceso el catálogo, un conjunto de datos, sus distribuciones y/o información adicional."@es ;
  rdfs:comment "Une page Web accessible par un navigateur Web donnant accès au catalogue, un jeu de données, ses distributions et/ou des informations additionnelles."@fr ;
  rdfs:comment "Webová stránka, na kterou lze pro získání přístupu ke katalogu, datové sadě, jejím distribucím a/nebo dalším informacím přistoupit webovým prohlížečem."@cs ;
  rdfs:comment "Μία ιστοσελίδα πλοηγίσιμη μέσω ενός φυλλομετρητή (Web browser) που δίνει πρόσβαση στο σύνολο δεδομένων, τις διανομές αυτού ή/και επιπρόσθετες πληροφορίες."@el ;
  rdfs:comment "صفحة وب يمكن من خلالها الوصول الى قائمة البيانات أو إلى معلومات إضافية متعلقة بها "@ar ;
  rdfs:comment "データセット、その配信および（または）追加情報にアクセスするためにウエブ・ブラウザでナビゲートできるウェブページ。"@ja ;
  rdfs:isDefinedBy <http://www.w3.org/TR/vocab-dcat/> ;
  rdfs:label "landing page"@en ;
  rdfs:label "page d'atterrissage"@fr ;
  rdfs:label "pagina di destinazione"@it ;
  rdfs:label "página de destino"@es ;
  rdfs:label "vstupní stránka"@cs ;
  rdfs:label "ιστοσελίδα αρχικής πρόσβασης"@el ;
  rdfs:label "صفحة وصول"@ar ;
  rdfs:label "ランディング・ページ"@ja ;
  rdfs:range foaf:Document ;
  rdfs:subPropertyOf foaf:page ;
  skos:scopeNote """If the distribution(s) are accessible only through a landing page (i.e. direct download
          URLs are not known), then the landing page link should be duplicated as accessURL on a distribution."""@en ;
  skos:scopeNote "Pokud je distribuce dostupná pouze přes vstupní stránku, t.j. přímý URL odkaz ke stažení není znám, URL přístupové stránky by mělo být duplikováno ve vlastnosti distribuce accessURL."@cs ;
  skos:scopeNote """Se la distribuzione è accessibile solo attraverso una pagina di destinazione (cioè, un URL di download diretto non è noto),
          il link alla pagina di destinazione deve essere duplicato come accessURL sulla distribuzione."""@it ;
  skos:scopeNote """Si la distribución es accesible solamente través de una página de aterrizaje (i.e., no se conoce una URL de descarga directa),
          entonces el enlance a la página de aterrizaje debe ser duplicado como accessURL sobre la distribución."""@es ;
  skos:scopeNote """Si la distribution est seulement accessible à travers une page d'atterrissage (exple. pas de connaissance d'URLS de téléchargement direct ), alors
						le lien de la page d'atterrissage doit être dupliqué comme accessURL sur la distribution."""@fr ;
  skos:scopeNote "Αν η/οι διανομή/ές είναι προσβάσιμη/ες μόνο μέσω μίας ιστοσελίδας αρχικής πρόσβασης (δηλαδή αν δεν υπάρχουν γνωστές διευθύνσεις άμεσης μεταφόρτωσης), τότε ο σύνδεσμος της ιστοσελίδας αρχικής πρόσβασης πρέπει να αναπαραχθεί ως accessURL σε μία διανομή."@el ;
  skos:scopeNote "ランディング・ページを通じてしか配信にアクセスできない場合（つまり、直接的なダウンロードURLが不明）には、配信におけるaccessURLとしてランディング・ページのリンクをコピーすべきです（SHOULD）。"@ja ;
.
dcat:mediaType
  rdf:type rdf:Property ;
  rdf:type owl:ObjectProperty ;
  rdfs:comment """Cette propriété doit être utilisée quand c'est définit le type de média de la distribution
					en IANA, sinon dct:format DOIT être utilisé avec différentes valeurs."""@fr ;
  rdfs:comment """Esta propiedad debe ser usada cuando está definido el tipo de media de la distribución
					en IANA, de otra manera dct:format puede ser utilizado con diferentes valores"""@es ;
  rdfs:comment "Il tipo di media della distribuzione come definito da IANA"@it ;
  rdfs:comment "Typ média distribuce definovaný v IANA."@cs ;
  rdfs:comment "The media type of the distribution as defined by IANA"@en ;
  rdfs:comment """Η ιδιότητα αυτή ΘΑ ΠΡΕΠΕΙ να χρησιμοποιείται όταν ο τύπος μέσου μίας διανομής είναι ορισμένος στο IANA, αλλιώς
          η ιδιότητα dct:format ΔΥΝΑΤΑΙ να χρησιμοποιηθεί με διαφορετικές τιμές."""@el ;
  rdfs:comment "يجب استخدام هذه الخاصية إذا كان نوع الملف معرف ضمن IANA"@ar ;
  rdfs:comment "このプロパティーは、配信のメディア・タイプがIANAで定義されているときに使用すべきで（SHOULD）、そうでない場合には、dct:formatを様々な値と共に使用できます（MAY）。"@ja ;
  rdfs:domain dcat:Distribution ;
  rdfs:isDefinedBy <http://www.w3.org/TR/vocab-dcat/> ;
  rdfs:label "media type"@en ;
  rdfs:label "tipo de media"@es ;
  rdfs:label "tipo di media"@it ;
  rdfs:label "typ média"@cs ;
  rdfs:label "type de média"@fr ;
  rdfs:label "τύπος μέσου"@el ;
  rdfs:label "نوع الميديا"@ar ;
  rdfs:label "メディア・タイプ"@ja ;
  rdfs:range dct:MediaType ;
  rdfs:subPropertyOf dct:format ;
  skos:editorialNote "Status: English Definition text modified by DCAT revision team, Italian and Czech translation provided, other translations pending. Note some inconsistency on def vs. usage"@en ;
  skos:changeNote "The range of dcat:mediaType has been tightened as part of the revision of DCAT."@en ;
  skos:changeNote "Obor hodnot dcat:mediaType byl zúžen v této revizi DCAT."@cs ;
  skos:scopeNote "This property SHOULD be used when the media type of the distribution is defined in the IANA media types registry https://www.iana.org/assignments/media-types/, otherwise dct:format MAY be used with different values."@en ;
  skos:scopeNote "Esta propiedad DEBERÍA usarse cuando el 'media type' de la distribución está definido en el registro IANA de 'media types' https://www.iana.org/assignments/media-types/, de lo contrario, dct:format PUEDE usarse con distintos valores."@es ;
  skos:scopeNote "Questa proprietà DEVE essere usata quando il tipo di media della distribuzione è definito nel registro dei tipi di media IANA https://www.iana.org/assignments/media-types/, altrimenti dct:format PUO 'essere usato con differenti valori"@it ;
  skos:scopeNote "Tato vlastnost BY MĚLA být použita, je-li typ média distribuce definován v registru IANA https://www.iana.org/assignments/media-types/. V ostatních případech MŮŽE být použita vlastnost dct:format s jinými hodnotami."@cs ;
.
dcat:compressFormat
  rdf:type rdf:Property ;
  rdf:type owl:ObjectProperty ;
  rdfs:comment "The compression format of the distribution in which the data is contained in a compressed form, e.g. to reduce the size of the downloadable file."@en ;
  rdfs:comment "El formato de la distribución en el que los datos están en forma comprimida, e.g. para reducir el tamaño del archivo a bajar."@es ;
  rdfs:comment "Il formato di compressione della distribuzione nel quale i dati sono in forma compressa, ad es. per ridurre le dimensioni del file da scaricare."@it ;
  rdfs:comment "Formát komprese souboru, ve kterém jsou data poskytována v komprimované podobě, např. ke snížení velikosti souboru ke stažení."@cs ;
  rdfs:domain dcat:Distribution ;
  rdfs:isDefinedBy <https://www.w3.org/TR/vocab-dcat-2/> ;
  rdfs:label "compression format"@en ;
  rdfs:label "formato de compresión"@es ;
  rdfs:label "formato di compressione"@it ;
  rdfs:label "formát komprese"@cs ;
  rdfs:range dct:MediaType ;
  rdfs:subPropertyOf dct:format ;
  skos:changeNote "New property added in DCAT 2.0."@en ;
  skos:changeNote "Nuova proprietà aggiunta in DCAT 2.0."@it ;
  skos:changeNote "Nueva propiedad agregada en DCAT 2.0."@es ;
  skos:changeNote "Nová vlastnost přidaná ve verzi DCAT 2.0"@cs ;
  skos:scopeNote "This property is to be used when the files in the distribution are compressed, e.g. in a ZIP file. The format SHOULD be expressed using a media type as defined by IANA media types registry https://www.iana.org/assignments/media-types/, if available."@en ;
  skos:scopeNote "Questa proprietà deve essere utilizzata quando i file nella distribuzione sono compressi, ad es. in un file ZIP. Il formato DOVREBBE essere espresso usando un tipo di media come definito dal registro dei tipi di media IANA https://www.iana.org/assignments/media-types/, se disponibile."@it ;
  skos:scopeNote "Esta propiedad se debe usar cuando los archivos de la distribución están comprimidos, por ejemplo en un archivo ZIP. El formato DEBERÍA expresarse usando un 'media type', tales como los definidos en el registro IANA de 'media types' https://www.iana.org/assignments/media-types/, si está disponibles."@es ;
  skos:scopeNote "Tato vlastnost se použije, když jsou soubory v distribuci komprimovány, např. v ZIP souboru. Formát BY MĚL být vyjádřen pomocí typu média definovaného v registru IANA https://www.iana.org/assignments/media-types/, pokud existuje."@cs ;
.
dcat:packageFormat
  rdf:type rdf:Property ;
  rdf:type owl:ObjectProperty ;
  rdfs:comment "The package format of the distribution in which one or more data files are grouped together, e.g. to enable a set of related files to be downloaded together."@en ;
  rdfs:comment "El formato del archivo en que se agrupan uno o más archivos de datos, e.g. para permitir que un conjunto de archivos relacionados se bajen juntos."@es ;
  rdfs:comment "Il formato di impacchettamento della distribuzione in cui uno o più file di dati sono raggruppati insieme, ad es. per abilitare un insieme di file correlati da scaricare insieme."@it ;
  rdfs:comment "Balíčkový formát souboru, ve kterém je jeden či více souborů seskupeno dohromady, např. aby bylo možné stáhnout sadu souvisejících souborů naráz."@cs ;
  rdfs:domain dcat:Distribution ;
  rdfs:isDefinedBy <https://www.w3.org/TR/vocab-dcat-2/> ;
  rdfs:label "packaging format"@en ;
  rdfs:label "formato de empaquetado"@es ;
  rdfs:label "formato di impacchettamento"@it ;
  rdfs:label "formát balíčku"@cs ;
  rdfs:range dct:MediaType ;
  rdfs:subPropertyOf dct:format ;
  skos:changeNote "New property added in DCAT 2.0."@en ;
  skos:changeNote "Nuova proprietà aggiunta in DCAT 2.0."@it ;
  skos:changeNote "Nueva propiedad agregada en DCAT 2.0."@es ;
  skos:changeNote "Nová vlastnost přidaná ve verzi DCAT 2.0"@cs ;
  skos:scopeNote "This property to be used when the files in the distribution are packaged, e.g. in a TAR file, a Frictionless Data Package or a Bagit file. The format SHOULD be expressed using a media type as defined by IANA media types registry https://www.iana.org/assignments/media-types/, if available."@en;
  skos:scopeNote "Esta propiedad se debe usar cuando los archivos de la distribución están empaquetados, por ejemplo en un archivo TAR, Frictionless Data Package o Bagit. El formato DEBERÍA expresarse usando un 'media type', tales como los definidos en el registro IANA de 'media types' https://www.iana.org/assignments/media-types/, si está disponibles."@es ;
  skos:scopeNote "Questa proprietà deve essere utilizzata quando i file nella distribuzione sono impacchettati, ad esempio in un file TAR, Frictionless Data Package o Bagit. Il formato DOVREBBE essere espresso utilizzando un tipo di supporto come definito dal registro dei tipi di media IANA https://www.iana.org/assignments/media-types/, se disponibili."@it ;
  skos:scopeNote "Tato vlastnost se použije, když jsou soubory v distribuci zabaleny, např. v souboru TAR, v balíčku Frictionless Data Package nebo v souboru Bagit. Formát BY MĚL být vyjádřen pomocí typu média definovaného v registru IANA https://www.iana.org/assignments/media-types/, pokud existuje."@cs ;
.
dcat:qualifiedRelation
  rdf:type owl:ObjectProperty ;
  rdfs:comment "Link to a description of a relationship with another resource."@en ;
  rdfs:comment "Enlace a una descripción de la relación con otro recurso."@es ;
  rdfs:comment "Link a una descrizione di una relazione con un'altra risorsa."@it ;
  rdfs:comment "Odkaz na popis vztahu s jiným zdrojem."@cs ;
  rdfs:domain dcat:Resource ;
  rdfs:label "qualified relation"@en ;
  rdfs:label "relación calificada"@es ;
  rdfs:label "relazione qualificata"@it ;
  rdfs:label "kvalifikovaný vztah"@cs ;
  rdfs:range dcat:Relationship ;
  skos:changeNote "New property added in DCAT 2.0."@en ;
  skos:changeNote "Propiedad nueva añadida en DCAT 2.0."@es ;
  skos:changeNote "Nuova proprietà aggiunta in DCAT 2.0."@it ;
  skos:changeNote "Nová vlastnost přidaná ve verzi DCAT 2.0"@cs ;
  skos:editorialNote "Introduced into DCAT to complement the other PROV qualified relations. "@en ;
  skos:editorialNote "Se incluyó en DCAT para complementar las relaciones calificadas disponibles en PROV. "@es ;
  skos:editorialNote "Introdotta in DCAT per integrare le altre relazioni qualificate di PROV."@it ;
  skos:editorialNote "Přidáno do DCAT k doplnění jiných kvalifikovaných vztahů ze slovníku PROV."@cs ;
  skos:scopeNote "Used to link to another resource where the nature of the relationship is known but does not match one of the standard Dublin Core properties (dct:hasPart, dct:isPartOf, dct:conformsTo, dct:isFormatOf, dct:hasFormat, dct:isVersionOf, dct:hasVersion, dct:replaces, dct:isReplacedBy, dct:references, dct:isReferencedBy, dct:requires, dct:isRequiredBy) or PROV-O properties (prov:wasDerivedFrom, prov:wasInfluencedBy, prov:wasQuotedFrom, prov:wasRevisionOf, prov:hadPrimarySource, prov:alternateOf, prov:specializationOf)."@en ;
  skos:scopeNote "Se usa para asociar con otro recurso para el cuál la naturaleza de la relación es conocida pero no es ninguna de las propiedades que provee el estándar Dublin Core (dct:hasPart, dct:isPartOf, dct:conformsTo, dct:isFormatOf, dct:hasFormat, dct:isVersionOf, dct:hasVersion, dct:replaces, dct:isReplacedBy, dct:references, dct:isReferencedBy, dct:requires, dct:isRequiredBy) or PROV-O properties (prov:wasDerivedFrom, prov:wasInfluencedBy, prov:wasQuotedFrom, prov:wasRevisionOf, prov:hadPrimarySource, prov:alternateOf, prov:specializationOf)."@es ;
  skos:scopeNote "Viene utilizzato per associarsi a un'altra risorsa nei casi per i quali la natura della relazione è nota ma non è alcuna delle proprietà fornite dallo standard Dublin Core (dct:hasPart, dct:isPartOf, dct:conformsTo, dct:isFormatOf, dct:hasFormat , dct:isVersionOf, dct:hasVersion, dct:replaces, dct:isReplacedBy, dct:references, dct:isReferencedBy, dct:require, dct:isRequiredBy) o dalle proprietà fornite da PROV-O (prov:wasDerivedFrom, prov:wasInfluencedBy, prov:wasQuotedFrom , prov:wasRevisionOf, prov:hadPrimarySource, prov:alternateOf, prov:specializationOf)."@it ;
  skos:scopeNote "Použito pro odkazování na jiný zdroj, kde druh vztahu je znám, ale neodpovídá standardním vlastnostem ze slovníku Dublin Core (dct:hasPart, dct:isPartOf, dct:conformsTo, dct:isFormatOf, dct:hasFormat, dct:isVersionOf, dct:hasVersion, dct:replaces, dct:isReplacedBy, dct:references, dct:isReferencedBy, dct:requires, dct:isRequiredBy) či slovníku PROV-O (prov:wasDerivedFrom, prov:wasInfluencedBy, prov:wasQuotedFrom, prov:wasRevisionOf, prov:hadPrimarySource, prov:alternateOf, prov:specializationOf)."@cs ;
.
dcat:record
  rdf:type rdf:Property ;
  rdf:type owl:ObjectProperty ;
  rdfs:comment "A record describing the registration of a single dataset or data service that is part of the catalog."@en ;
  rdfs:comment "Describe la registración de un conjunto de datos o un servicio de datos en el catálogo."@es ;
  rdfs:comment "Un record che descrive la registrazione di un singolo set di dati o di un servizio dati che fa parte del catalogo."@it ;
  rdfs:comment "Záznam popisující registraci jedné datové sady či datové služby jakožto součásti katalogu."@cs ;
  rdfs:comment "Propojuje katalog a jeho záznamy."@cs ;
  rdfs:comment "Relie un catalogue à ses registres"@fr ;
  rdfs:comment "Συνδέει έναν κατάλογο με τις καταγραφές του."@el ;
  rdfs:comment "تربط الفهرس بسجل ضمنه"@ar ;
  rdfs:comment "カタログの一部であるカタログ・レコード。"@ja ;
  rdfs:domain dcat:Catalog ;
  rdfs:isDefinedBy <http://www.w3.org/TR/vocab-dcat/> ;
  rdfs:label "record"@en ;
  rdfs:label "record"@it ;
  rdfs:label "registre"@fr ;
  rdfs:label "registro"@es ;
  rdfs:label "záznam"@cs ;
  rdfs:label "καταγραφή"@el ;
  rdfs:label "سجل"@ar ;
  rdfs:label "カタログ・レコード"@ja ;
  rdfs:range dcat:CatalogRecord ;
  skos:editorialNote "Status: English, Italian, Spanish and Czech Definitions modified by DCAT revision team, other translations pending."@en ;
.
dcat:servesDataset
  rdf:type owl:ObjectProperty ;
  rdfs:comment "A collection of data that this DataService can distribute"@en ;
  rdfs:comment "Una raccolta di dati che questo DataService può distribuire"@it ;
  rdfs:comment "Una colección de datos que este Servicio de Datos puede distribuir."@es ;
  rdfs:comment "Kolekce dat, kterou je tato Datová služba schopna poskytnout"@cs ;
  rdfs:domain dcat:DataService ;
  rdfs:label "serves dataset"@en ;
  rdfs:label "serve set di dati"@it ;
  rdfs:label "provee conjunto de datos"@es ;
  rdfs:label "poskytuje datovou sadu"@cs ;
  rdfs:range dcat:Dataset ;
  skos:changeNote "New property in DCAT 2.0."@en ;
  skos:changeNote "Nuova proprietà in DCAT 2.0."@it ;
  skos:changeNote "Nueva propiedad agregada en DCAT 2.0."@es ;
  skos:changeNote "Nová vlastnost přidaná ve verzi DCAT 2.0"@cs ;
.
dcat:service
  rdf:type owl:ObjectProperty ;
  rdfs:comment "A site or endpoint that is listed in the catalog."@en ;
  rdfs:comment "Un sitio o 'endpoint' que está listado en el catálogo."@es ;
  rdfs:comment "Un sito o endpoint elencato nel catalogo."@it ;
  rdfs:comment "Umístění či přístupový bod registrovaný v katalogu."@cs ;
  rdfs:domain dcat:Catalog ;
  rdfs:label "service"@en ;
  rdfs:label "servicio"@es ;
  rdfs:label "servizio"@it ;
  rdfs:label "služba"@cs ;
  rdfs:range dcat:DataService ;
  rdfs:subPropertyOf dct:hasPart ;
  rdfs:subPropertyOf rdfs:member ;
  skos:changeNote "New property added in DCAT 2.0."@en ;
  skos:changeNote "Nueva propiedad añadida en DCAT 2.0."@es ;
  skos:changeNote "Nuova proprietà aggiunta in DCAT 2.0."@it ;
  skos:changeNote "Nová vlastnost přidaná ve verzi DCAT 2.0"@cs ;
.
dcat:spatialResolutionInMeters
  rdf:type owl:DatatypeProperty ;
  rdfs:comment "minimum spatial separation resolvable in a dataset, measured in meters"@en-US ;
  rdfs:comment "minimum spatial separation resolvable in a dataset, measured in metres"@en-GB ;
  rdfs:comment "mínima separacíon espacial disponible en un conjunto de datos, medida en metros"@es ;
  rdfs:comment "separazione spaziale minima risolvibile in un set di dati, misurata in metri"@it ;
  rdfs:comment "minimální prostorový rozestup rozeznatelný v datové sadě, měřeno v metrech"@cs ;
  rdfs:label "spatial resolution (meters)"@en-US ;
  rdfs:label "spatial resolution (metres)"@en-GB ;
  rdfs:label "resolución espacial (metros)"@es ;
  rdfs:label "risoluzione spaziale (metros)"@it ;
  rdfs:label "prostorové rozlišení (metry)"@cs ;
  rdfs:range xsd:decimal ;
  skos:changeNote "New property added in DCAT 2.0."@en ;
  skos:changeNote "Nueva propiedad añadida en DCAT 2.0."@es ;
  skos:changeNote "Nuova proprietà aggiunta in DCAT 2.0."@it ;
  skos:changeNote "Nová vlastnost přidaná ve verzi DCAT 2.0"@cs ;
  skos:editorialNote "Might appear in the description of a Dataset or a Distribution, so no domain is specified"@en ;
  skos:editorialNote "Může se vyskytnout v popisu Datové sady nebo Distribuce, takže nebyl specifikován definiční obor"@cs ;
  skos:scopeNote "If the dataset is an image or grid this should correspond to the spacing of items. For other kinds of spatial dataset, this property will usually indicate the smallest distance between items in the dataset. "@en ;
  skos:scopeNote "Si el conjunto de datos es una imágen o grilla, esta propiedad corresponde al espaciado de los elementos. Para otro tipo de conjunto de datos espaciales, esta propieda usualmente indica la menor distancia entre los elementos de dichos datos."@es ;
  skos:scopeNote "Se il set di dati è un'immagine o una griglia, questo dovrebbe corrispondere alla spaziatura degli elementi. Per altri tipi di set di dati spaziali, questa proprietà di solito indica la distanza minima tra gli elementi nel set di dati."@it ;
  skos:scopeNote "Pokud je datová sada obraz či mřížka, měla by tato vlastnost odpovídat rozestupu položek. Pro ostatní druhy prostorových datových sad bude tato vlastnost obvykle indikovat nejmenší vzdálenost mezi položkami této datové sady."@cs ;
  skos:scopeNote "Alternative spatial resolutions might be provided as different dataset distributions"@en ;
  skos:scopeNote "Distintas distribuciones de un conjunto de datos pueden tener resoluciones espaciales diferentes"@es ;
  skos:scopeNote "Risoluzioni spaziali alternative possono essere fornite come diverse distribuzioni di set di dati"@it ;
  skos:scopeNote "Různá prostorová rozlišení mohou být poskytována jako různé distribuce datové sady"@cs ;
.
dcat:startDate
  rdfs:label "start date"@en;
  rdfs:label "datum začátku"@cs;
  rdf:type rdf:Property ;
  rdf:type owl:DatatypeProperty ;
  rdfs:domain dct:PeriodOfTime ;
  rdfs:range rdfs:Literal ;
  skos:definition "The start of the period"@en ;
  skos:definition "El comienzo del período "@es ;
  skos:definition "Začátek doby trvání"@cs ;
  skos:changeNote "New property added in DCAT 2.0."@en ;
  skos:changeNote "Nueva propiedad agregada en DCAT 2.0."@es ;
  skos:changeNote "Nová vlastnost přidaná ve verzi DCAT 2.0"@cs ;
  skos:scopeNote "The range of this property is intentionally generic, with the purpose of allowing different level of temporal precision for specifying the start of a period. E.g., it can be expressed with a date (xsd:date), a date and time (xsd:dateTime), or a year (xsd:gYear)."@en ;
  skos:scopeNote "El rango de esta propiedad es intencionalmente genérico con el propósito de permitir distintos niveles de precisión temporal para especificar el comienzo de un período. Por ejemplo, puede expresarse como una fecha (xsd:date), una fecha y un tiempo (xsd:dateTime), o un año (xsd:gYear)."@es ;
  skos:scopeNote "Obor hodnot této vlastnosti je úmyslně obecný, aby umožnil různé úrovně časového rozlišení pro specifikaci začátku doby trvání. Ten může být kupříkladu vyjádřen datumem (xsd:date), datumem a časem (xsd:dateTime) či rokem (xsd:gYear)."@cs ;
.
dcat:temporalResolution
  rdf:type owl:DatatypeProperty ;
  rdfs:comment "minimum time period resolvable in a dataset"@en ;
  rdfs:comment "período de tiempo mínimo en el conjunto de datos"@es ;
  rdfs:comment "periodo di tempo minimo risolvibile in un set di dati"@it;
  rdfs:comment "minimální doba trvání rozlišitelná v datové sadě"@cs ;
  rdfs:label "temporal resolution"@en ;
  rdfs:label "resolución temporal"@es ;
  rdfs:label "risoluzione temporale"@it ;
  rdfs:label "časové rozlišení"@cs ;
  rdfs:range xsd:duration ;
  skos:changeNote "New property added in DCAT 2.0."@en ;
  skos:changeNote "Nueva propiedad añadida en DCAT 2.0."@es ;
  skos:changeNote "Nuova proprietà aggiunta in DCAT 2.0."@it ;
  skos:changeNote "Nová vlastnost přidaná ve verzi DCAT 2.0"@cs ;
  skos:editorialNote "Might appear in the description of a Dataset or a Distribution, so no domain is specified"@en ;
  skos:editorialNote "Může se vyskytnout v popisu Datové sady nebo Distribuce, takže nebyl specifikován definiční obor"@cs ;
  skos:scopeNote "If the dataset is a time-series this should correspond to the spacing of items in the series. For other kinds of dataset, this property will usually indicate the smallest time difference between items in the dataset. "@en ;
  skos:scopeNote "Si el conjunto de datos es una serie temporal, debe corresponder al espaciado de los elementos de la serie. Para otro tipo de conjuntos de datos, esta propiedad indicará usualmente la menor diferencia de tiempo entre elementos en el dataset."@es ;
  skos:scopeNote "Se il set di dati è una serie temporale, questo dovrebbe corrispondere alla spaziatura degli elementi della serie. Per altri tipi di set di dati, questa proprietà di solito indica la più piccola differenza di tempo tra gli elementi nel set di dati."@it ;
  skos:scopeNote "Pokud je datová sada časovou řadou, měla by tato vlastnost odpovídat rozestupu položek v řadě. Pro ostatní druhy datových sad bude tato vlastnost obvykle indikovat nejmenší časovou vzdálenost mezi položkami této datové sady."@cs ;
  skos:scopeNote "Alternative temporal resolutions might be provided as different dataset distributions"@en ;
  skos:scopeNote "Distintas distribuciones del conjunto de datos pueden tener resoluciones temporales diferentes."@es ;
  skos:scopeNote "Risoluzioni temporali alternative potrebbero essere fornite come diverse distribuzioni di set di dati"@it ;
  skos:scopeNote "Různá časová rozlišení mohou být poskytována jako různé distribuce datové sady"@cs ;
.
dcat:theme
  rdf:type rdf:Property ;
  rdf:type owl:ObjectProperty ;
  rdfs:comment "A main category of the resource. A resource can have multiple themes."@en ;
  rdfs:comment "Hlavní téma zdroje. Zdroj může mít více témat."@cs ;
  rdfs:comment "La categoria principale della risorsa. Una risorsa può avere più temi."@it ;
  rdfs:comment "La categoría principal del recurso. Un recurso puede tener varios temas."@es ;
  rdfs:comment "La catégorie principale de la ressource. Une ressource peut avoir plusieurs thèmes."@fr ;
  rdfs:comment "Η κύρια κατηγορία του συνόλου δεδομένων. Ένα σύνολο δεδομένων δύναται να έχει πολλαπλά θέματα."@el ;
  rdfs:comment "التصنيف الرئيسي لقائمة البيانات. قائمة البيانات يمكن أن تملك أكثر من تصنيف رئيسي واحد."@ar ;
  rdfs:comment "データセットの主要カテゴリー。データセットは複数のテーマを持つことができます。"@ja ;
  rdfs:isDefinedBy <http://www.w3.org/TR/vocab-dcat/> ;
  rdfs:label "tema"@es ;
  rdfs:label "tema"@it ;
  rdfs:label "theme"@en ;
  rdfs:label "thème"@fr ;
  rdfs:label "téma"@cs ;
  rdfs:label "Θέμα"@el ;
  rdfs:label "التصنيف"@ar ;
  rdfs:label "テーマ/カテゴリー"@ja ;
  rdfs:range skos:Concept ;
  rdfs:subPropertyOf dct:subject ;
  skos:editorialNote "Status: English Definition text modified by DCAT revision team, all except for Italian and Czech translations are pending."@en ;
  skos:scopeNote """El conjunto de skos:Concepts utilizados para categorizar los recursos están organizados en
          un skos:ConceptScheme que describe todas las categorías y sus relaciones en el catálogo"""@es ;
  skos:scopeNote "Il set di concetti skos usati per categorizzare le risorse sono organizzati in skos:ConceptScheme che descrive tutte le categorie e le loro relazioni nel catalogo."@it ;
  skos:scopeNote "Sada instancí třídy skos:Concept použitá pro kategorizaci zdrojů je organizována do schématu konceptů skos:ConceptScheme, které popisuje všechny kategorie v katalogu a jejich vztahy."@cs ;
  skos:scopeNote "The set of skos:Concepts used to categorize the resources are organized in a skos:ConceptScheme describing all the categories and their relations in the catalog."@en ;
  skos:scopeNote """Un ensemble de skos:Concepts utilisés pour catégoriser les ressources sont organisés en
						un skos:ConceptScheme décrivqnt toutes les catégories et ses relations dans le catalogue."""@fr ;
  skos:scopeNote """Το σετ των skos:Concepts που χρησιμοποιείται για να κατηγοριοποιήσει τα σύνολα δεδομένων είναι οργανωμένο εντός
          ενός skos:ConceptScheme που περιγράφει όλες τις κατηγορίες και τις σχέσεις αυτών στον κατάλογο."""@el ;
  skos:scopeNote "データセットを分類するために用いられるskos:Conceptの集合は、カタログのすべてのカテゴリーとそれらの関係を記述しているskos:ConceptSchemeで組織化されます。"@ja ;
.
dcat:themeTaxonomy
  rdf:type rdf:Property ;
  rdf:type owl:ObjectProperty ;
  rdfs:comment "El sistema de organización del conocimiento utilizado para clasificar conjuntos de datos de catálogos."@es ;
  rdfs:comment "Il sistema di organizzazione della conoscenza (KOS) usato per classificare i dataset del catalogo."@it ;
  rdfs:comment "Le systhème d'ogranisation de connaissances utilisé pour classifier les jeux de données du catalogue."@fr ;
  rdfs:comment "Systém organizace znalostí (KOS) použitý pro klasifikaci datových sad v katalogu."@cs ;
  rdfs:comment "The knowledge organization system (KOS) used to classify catalog's datasets."@en ;
  rdfs:comment "Το σύστημα οργάνωσης γνώσης που χρησιμοποιείται για την κατηγοριοποίηση των συνόλων δεδομένων του καταλόγου."@el ;
  rdfs:comment "لائحة التصنيفات المستخدمه لتصنيف قوائم البيانات ضمن الفهرس"@ar ;
  rdfs:comment "カタログのデータセットを分類するために用いられる知識組織化体系（KOS；knowledge organization system）。"@ja ;
  rdfs:domain dcat:Catalog ;
  rdfs:isDefinedBy <http://www.w3.org/TR/vocab-dcat/> ;
  rdfs:label "tassonomia dei temi"@it ;
  rdfs:label "taxonomie de thèmes"@fr ;
  rdfs:label "taxonomie témat"@cs ;
  rdfs:label "taxonomía de temas"@es ;
  rdfs:label "theme taxonomy"@en ;
  rdfs:label "Ταξινομία θεματικών κατηγοριών."@el ;
  rdfs:label "قائمة التصنيفات"@ar ;
  rdfs:label "テーマ"@ja ;
#  rdfs:range skos:ConceptScheme ;
  rdfs:range rdfs:Resource ;
  sdo:rangeIncludes skos:ConceptScheme , skos:Collection , owl:Ontology ;
  skos:scopeNote "It is recommended that the taxonomy is organized in a skos:ConceptScheme, skos:Collection, owl:Ontology or similar, which allows each member to be denoted by an IRI and published as linked-data."@en ;
  skos:scopeNote "Se recomienda que la taxonomía se organice como un skos:ConceptScheme, skos:Collection, owl:Ontology o similar, los cuáles permiten que cada miembro se denote con una IRI y se publique como datos enlazados."@es ;
  skos:scopeNote "Je doporučeno, aby byla taxonomie vyjádřena jako skos:ConceptScheme, skos:Collection, owl:Ontology nebo podobné, aby mohla být každá položka identifikována pomocí IRI a publikována jako propojená data."@cs ;
.
dct:PeriodOfTime
  skos:definition "An interval of time that is named or defined by its start and end dates."@en ;
  skos:definition "In the context of DCAT 2.0, an interval of time that is named or defined by its start and end."@en ;
  skos:definition "En el contexto de DCAT 2.0, un interválo de tiempo que se nombra o define por su principio y fin."@es ;
  skos:definition "En el contexto de DCAT 2.0, časový interval který je pojmenovaný, nebo určený svým začátkem a koncem."@cs ;
  skos:changeNote "Class added in this context in DCAT 2.0."@en ;
  skos:changeNote "En el contexto de DCAT 2.0, esta clase se agregó en este contexto en DCAT 2.0."@es ;
  skos:changeNote "Třída v tomto kontextu byla přidána ve verzi DCAT 2.0"@cs ;
  skos:scopeNote "In the context of DCAT 2.0, the start and end of the interval may be given by using properties dcat:startDate or time:hasBeginning, and dcat:endDate or time:hasEnd, respectively. The interval can also be open - i.e., it can have just a start or just an end."@en ;
  skos:scopeNote "En el contexto de DCAT 2.0, el comienzo y fin de un intervalo pueden representarse usando las propiedades dcat:startDate o time:hasBeginning, y dcat:endDate o time:hasEnd, respectivamente. El interválo también puede ser un interválo abierto - es decir, puede tener sólo un comienzo o un fin."@es ;
  skos:scopeNote "En el contexto de DCAT 2.0, začátek a konec intervalu může být dán vlastnostmi dcat:startDate či time:hasBeginning a dcat:endDate či time:hasEnd. Interval také může být otevřený, tj. může mít pouze začátek či pouze konec."@cs ;
.
dct:Location
  skos:definition "A spatial region or named place."@en ;
  skos:definition "A spatial region or named place."@es ;
  skos:definition "Prostorová oblast či pojmenované místo."@cs ;
  skos:changeNote "Class added in this context in DCAT 2.0."@en ;
  skos:changeNote "Esta clase se agregó en este contexto en DCAT 2.0."@es ;
  skos:changeNote "Třída v tomto kontextu byla přidána ve verzi DCAT 2.0"@cs ;
  skos:scopeNote "In the context of DCAT 2.0, for an extensive geometry (i.e., a set of coordinates denoting the vertices of the relevant geographic area), the property locn:geometry [[LOCN]] SHOULD be used."@en ;
  skos:scopeNote "En el contexto de DCAT 2.0, para una geometría extensiva (es decir, un conjunto de coordinadas que denotan los vértices de un área geográfica), DEBE usarse la propiedad locn:geometry [[LOCN]]."@es ;
  skos:scopeNote "En el contexto de DCAT 2.0, pro rozsáhlé geometrie (tj. sady souřadnic určujících relevantní geografickou oblast) BY MĚLA být použita vlastnost locn:geometry [[LOCN]]."@cs ;
  skos:scopeNote "In the context of DCAT 2.0, for a geographic bounding box delimiting a spatial area the property dcat:bbox SHOULD be used."@en ;
  skos:scopeNote "En el contexto de DCAT 2.0, para un cuadro delimitador geográfico que delimita un área espacial se DEBE usar la propiedad dcat:bbox."@es ;
  skos:scopeNote "En el contexto de DCAT 2.0, pro geografický rámec ohraničující prostorové oblasti BY MĚLA být použita vlastnost dcat:bbox."@cs ;
  skos:scopeNote "In the context of DCAT 2.0, for the geographic center of a spatial area, or another characteristic point, the property dcat:centroid SHOULD be used."@en ;
  skos:scopeNote "En el contexto de DCAT 2.0, para el centro geográfico de un área espacial, o algún otro punto característico, se DEBE usar la propriedad dcat:centroid."@es ;
  skos:scopeNote "En el contexto de DCAT 2.0, pro geografický střed prostorové oblasti či jiný charakteristický bod BY MĚLA být použita vlastnost dcat:centroid."@cs ;
.
dct:accessRights
  skos:definition "Information about who can access the resource or an indication of its security status."@en ;
#  skos:scopeNote "In the context of DCAT 2.0 dcat:Resource, a rights statement that concerns how the resource is accessed."@en ;
#  skos:scopeNote "En el contexto de DCAT 2.0 dcat:Resource, una declaración de derechos sobre cómo se puede acceder el recurso."@es ;
#  skos:scopeNote "V kontextu DCAT 2.0 dcat:Resource, podmínky užití řešící způsob přístupu ke zdroji."@cs ;
  skos:definition "In the context of DCAT 2.0 dcat:Distribution, a rights statement that concerns how the distribution is accessed."@en ;
  skos:definition "En el contexto de DCAT 2.0 dcat:Distribution, una declaración de derechos sobre cómo se puede acceder la distribución."@es ;
  skos:definition "V kontextu DCAT 2.0 dcat:Distribution, podmínky užití řešící způsob přístupu k distribuci."@cs ;
  skos:scopeNote "In the context of DCAT 2.0 dcat:Resource, information about licenses and rights MAY be provided for the Resource. See also guidance in the section 'License and rights statements'."@en ;
  skos:scopeNote "En el contexto de DCAT 2.0 dcat:Resource, información sobre las licencias y derechos que PUEDEN proveerse para un Recurso. Ver también la información en la sección 'License and rights statements'."@es ;
  skos:scopeNote "V kontextu DCAT 2.0 dcat:Resource, pro Zdroj MŮŽE BÝT uvedena informace o podmínkách užití (licencích a právech). Viz návod v sekci 'License and rights statements'."@cs ;
  skos:scopeNote "In the context of DCAT 2.0 dcat:Distribution, information about licenses and rights MAY be provided for the Distribution. See also guidance in the section 'License and rights statements'."@en ;
  skos:scopeNote "En el contexto de DCAT 2.0 dcat:Distribution, información sobre licencias y derechos que PUEDE proveerse para una Distribución. Ver también la información en la sección 'License and rights statements'."@es ;
  skos:scopeNote "V kontextu DCAT 2.0 dcat:Distribution, pro Distribuci MŮŽE BÝT uvedena informace o podmínkách užití (licencích a právech). Viz návod v sekci 'License and rights statements'."@cs ;
  skos:scopeNote "In the context of DCAT 2.0 dcat:DataService, access Rights MAY include information regarding access or restrictions based on privacy, security, or other policies."@en ;
  skos:scopeNote "En el contexto de DCAT 2.0 dcat:DataService, los derechos de acceso PUEDEN incluir información sobre acceso o restricciones basadas en privacidad, seguridad, u otras reglamentaciones."@es ;
  skos:scopeNote "V kontextu DCAT 2.0 dcat:DataService, podmínky užití MOHOU obsahovat informace o přístupu nebo omezení z hlediska soukromí, bezpečnosti nebo jiných pravidel."@cs ;
.
dct:accrualPeriodicity
  skos:definition "The frequency with which items are added to a collection."@en ;
  skos:definition "In the context of DCAT 2.0, the frequency at which dataset is published."@en ;
  skos:definition "En el contexto de DCAT 2.0, la frecuencia con que se publica el conjunto de datos."@es ;
  skos:definition "V kontextu DCAT 2.0, frekvence publikace datové sady."@cs ;
  skos:scopeNote "In the context of DCAT 2.0, the value of dct:accrualPeriodicity gives the rate at which the dataset-as-a-whole is updated. This may be complemented by dcat:temporalResolution to give the time between collected data points in a time series."@en ;
  skos:scopeNote "En el contexto de DCAT 2.0, el valor de dct:accrualPeriodicity da la tasa de actualización del conjunto de datos como entidad. Esto puede complementarse con dcat:temporalResolution para dar el tiempo entre los puntos en que se recopilan los datos en una serie temporal."@es ;
  skos:scopeNote "V kontextu DCAT 2.0, hodnota dct:accrualPeriodicity udává frekvenci, se kterou se aktualizuje datová sada jako celek. Toto může být doplněno vlastností dcat:temporalResolution pro udání času mezi jednotlivými body v časové řadě."@cs ;
.
dct:conformsTo
  skos:definition "An established standard to which the described resource conforms."@en ;
  skos:definition "Un estándar establecido al cuál se ajusta el recurso descripto."@es ;
  skos:definition "In the context of DCAT 2.0 dcat:Distribution, an established standard to which the distribution conforms."@en ;
  skos:definition "En el contexto de DCAT 2.0 dcat:Distribution, un estándar establecido al cuál se ajusta la distribución."@es ;
  skos:definition "V kontextu DCAT 2.0 dcat:Distribution, uznávaný standard, kterým se popisovaný zdroj řídí."@cs ;
  skos:scopeNote "In the context of DCAT 2.0 dcat:Resource, this property SHOULD be used to indicate the model, schema, ontology, view or profile that the cataloged resource content conforms to."@en ;
  skos:scopeNote "En el contexto de DCAT 2.0 dcat:Resource, esta propiedad DEBERÍA usarse para indicar el modelo, esquema, ontología, vista or perfil al que se ajusta el recurso catalogado."@es ;
  skos:scopeNote "V kontextu DCAT 2.0 dcat:Resource, tato vlastnost BY MĚLA být použita k udání modelu, schématu, ontologie, pohledu nebo profilu, kterému katalogizovaný zdroj odpovídá."@cs ;
  skos:scopeNote "In the context of DCAT 2.0 dcat:Distribution, this property SHOULD be used to indicate the model, schema, ontology, view or profile that this representation of a dataset conforms to. This is (generally) a complementary concern to the media-type or format."@en ;
  skos:scopeNote "En el contexto de DCAT 2.0 dcat:Distribution, esta propiedad DEBERÍA usarse para indicar el modelo, esquema, ontología, vista or perfil al que se ajusta esta representación del conjunto de datos. Este es (generalmente) un asunto complementario al de 'media type' o formato."@es ;
  skos:scopeNote "V kontextu DCAT 2.0 dcat:Distribution, tato vlastnost BY MĚLA být použita k udání modelu, schématu, ontologie, pohledu nebo profilu, kterému tato reprezentace datové sady odpovídá. Toto (obvykle) doplňuje typ média či formát."@cs ;
  skos:changeNote "Property added in this context in DCAT 2.0."@en ;
  skos:changeNote "Esta propiedad fue agregada en DCAT 2.0."@es ;
  skos:changeNote "Vlastnost v tomto kontextu byla přidána ve verzi DCAT 2.0"@cs ;
.
dct:creator
  skos:definition "An entity primarily responsible for making the resource."@en ;
  skos:definition "In the context of DCAT 2.0, the entity responsible for producing the resource."@en ;
  skos:definition "En el contexto de DCAT 2.0, la entidad responsable de producier el recurso."@es ;
  skos:definition "V kontextu DCAT 2.0, entita zodpovědná za tvorbu zdroje."@cs ;
  skos:scopeNote "In the context of DCAT 2.0, resources of type foaf:Agent are recommended as values for this property."@en ;
  skos:scopeNote "En el contexto de DCAT 2.0, se recomienda que los valores de esta propiedad sean recurso de tipo foaf:Agent."@es ;
  skos:scopeNote "V kontextu DCAT 2.0, doporučovanou hodnotou této vlastnosti jsou zdroje typu foaf:Agent."@cs ;
  skos:changeNote "Property added in this context in DCAT 2.0, specifically to address data citation requirements."@en ;
  skos:changeNote "Esta propiedad fue agregada en DCAT 2.0, específicamente para tratar los requerimientos de cita de datos."@es ;
  skos:changeNote "Vlastnost v tomto kontextu byla přidána ve verzi DCAT 2.0 zejména za účelem uspokojení požadavků na citace dat."@cs ;
.
dct:description
  skos:definition "An account of the resource."@en ;
  skos:definition "In the context of DCAT 2.0, a free-text account of the item."@en ;
  skos:definition "En el contexto de DCAT 2.0, una explicación en texto sobre el ítem."@es ;
  skos:definition "V kontextu DCAT 2.0, popis položky pomocí volného textu."@cs ;
.
dct:format
  skos:definition "The file format, physical medium, or dimensions of the resource."@en ;
  skos:definition "In the context of DCAT 2.0, the file format of the distribution."@en ;
  skos:definition "En el contexto de DCAT 2.0, el formato del archivo de la distribución."@es ;
  skos:definition "V kontextu DCAT 2.0, formát souboru distribuce."@cs ;
  skos:scopeNote "In the context of DCAT 2.0, dcat:mediaType SHOULD be used if the type of the distribution is defined by IANA [IANA-MEDIA-TYPES]."@en ;
  skos:scopeNote "En el contexto de DCAT 2.0, dcat:mediaType DEBERÍA usarse si el tipo de distribución se define por IANA [IANA-MEDIA-TYPES]."@es ;
  skos:scopeNote "V kontextu DCAT 2.0, pokud je typ distribuce definován IANA [IANA-MEDIA-TYPES], MĚLA BY být použita vlastnost dcat:mediaType."@cs ;
.
dct:hasPart
  skos:definition "A related resource that is included either physically or logically in the described resource."@en ;
  skos:definition "In the context of DCAT 2.0 dcat:Catalog, an item that is listed in the catalog."@en ;
  skos:scopeNote "In the context of DCAT 2.0, this is the most general predicate for membership of a catalog. Use of a more specific sub-property is recommended when available."@en ;
  skos:scopeNote "En el contexto de DCAT 2.0, este es el predicado más general para la membresía en un catálogo. Se recomienda usar una sub-propiedad más específica si hay una disponible."@es ;
  skos:scopeNote "V kontextu DCAT 2.0, toto je nejobecnější predikát pro příslušnost do katalogu. Pokud je to možné, doporučuje se použít konkrétnější vztah."@cs ;
  skos:scopeNote "In the context of DCAT 2.0, see also: Sub-properties of dct:hasPart; in particular dcat:dataset, dcat:catalog, dcat:service."@en ;
  skos:scopeNote "En el contexto de DCAT 2.0, vea también: sub-propiedades de dct:hasPart; en particular dcat:dataset, dcat:catalog, dcat:service."@es ;
  skos:scopeNote "V kontextu DCAT 2.0, viz také: Podvlastnosti dct:hasPart; zejména dcat:dataset, dcat:catalog, dcat:service."@cs ;
.
dct:identifier
  skos:definition "An unambiguous reference to the resource within a given context."@en ;
  skos:definition "In the context of DCAT 2.0, a unique identifier of the item."@en ;
  skos:definition "En el contexto de DCAT 2.0, un identificador único para el ítem."@es ;
  skos:definition "V kontextu DCAT 2.0, unikátní identifikátor položky."@cs ;
  skos:scopeNote "In the context of DCAT 2.0, the identifier might be used as part of the URI of the item, but still having it represented explicitly is useful."@en ;
  skos:scopeNote "En el contexto de DCAT 2.0, el identificador puede usarse como parte de la URI del ítem, pero es útil tenerlo representado de forma explícita."@es ;
  skos:scopeNote "V kontextu DCAT 2.0, identifikátor může být použit jako součást IRI položky. I přesto je užitečné mít jeho explicitní reprezentaci."@cs ;
.
dct:isReferencedBy
  skos:definition "A related resource that references, cites, or otherwise points to the described resource."@en ;
  skos:definition "In the context of DCAT 2.0, a related resource, such as a publication, that references, cites, or otherwise points to the catalogued resource.."@en ;
  skos:definition "En el contexto de DCAT 2.0, un recurso relacionado, como por ejemplo una publicación, que referencia, cita, o apunta al recurso del catálogo."@es ;
  skos:definition "V kontextu DCAT 2.0, související zdroj, např. publikace, který se odkazuje, cituje nebo jinak ukazuje na katalogizovaný zdroj."@cs ;
  skos:scopeNote "In the context of DCAT 2.0, in relation to the use case of data citation, when the catalogued resource is a dataset, the dct:isReferencedBy property allows to relate the dataset to the resources (such as scholarly publications) that cite or point to the dataset. Multiple dct:isReferencedBy properties can be used to indicate the dataset has been referenced by multiple publications, or other resources."@en ;
  skos:scopeNote "En el contexto de DCAT 2.0, en relación al caso de uso sobre cita de datos, cuando el recurso catalogado es un conjunto de datos, la propiedad dct:isReferencedBy permite relacionar el conjunto de datos a publicaciones que citan o apuntan al conjunto de datos. Se pueden utilizar múltiples propiedades dct:isReferencedBy para indicar que el conjunto de datos se ha referenciado en múltiples publicaciones u otros recursos."@es ;
  skos:scopeNote "V kontextu DCAT 2.0, ohledně případu užití vztahujícího se k citaci dat, pokud je katalogizovaný zdroj datovou sadou, vlastnost dct:isReferencedBy umožňuje vztáhnout tuto datovou sadu ke zdroji (např. odborné publikaci) která ji cituje nebo na ni odkazuje. dct:isReferencedBy lze užít vícenásobně pro zaznamenání faktu, že datová sada byla odkazována z více publikací nebo jiných zdrojů."@cs ;
  skos:changeNote "Property added in this context in DCAT 2.0."@en ;
  skos:changeNote "En el contexto de DCAT 2.0, esta propiedad fue agregada en DCAT 2.0."@es ;
  skos:changeNote "Vlastnost byla v tomto kontextu přidána ve verzi DCAT 2.0"@cs ;
  skos:scopeNote "In the context of DCAT 2.0, this property is used to associate a resource to the catalogued resource (of type dcat:Resource) in question. For other relations to resources not covered with this property, the more generic property dcat:qualifiedRelation can be used. See also the section about § 9. Qualified relations ."@en ;
  skos:scopeNote "En el contexto de DCAT 2.0, esta propiedad se usa para asociar un recurso a un elemento del catálogo  (de tipo dcat:Resource). Para representar otro tipo de associaciones a recursos, se puede utilizar la propiedad más genérica dcat:qualifiedRelation. Para más detalle, ver la sección en relaciones calificadas de la especificación."@es ;
  skos:scopeNote "V kontextu DCAT 2.0,tato vlastnost je použita k přiřazení zdroje ke katalogizovanému zdroji (typu dcat:Resource). Pro jiné typy vztahů ke zdrojům, které nejsou touto vlastností pokryty, může být použita obecnější vlastnost dcat:qualifiedRelation. Viz také sekce 9. 'Qualified relations'."@cs ;
.
dct:issued
  skos:definition "Date of formal issuance (e.g., publication) of the resource."@en ;
  skos:definition "In the context of DCAT 2.0 dcat:CatalogRecord, the date of listing (i.e. formal recording) of the corresponding dataset or service in the catalog."@en ;
  skos:definition "En el contexto de DCAT 2.0 dcat:CatalogRecord, la fecha en que lista (es decir, se registra formalmente) el conjunto de datos o servicio correspondiente en el catálogo."@es ;
  skos:definition "V kontextu DCAT 2.0 dcat:CatalogRecord, datum zanesení datové sady nebo služby do katalogu."@cs ;
  skos:definition "In the context of DCAT 2.0 dcat:Distribution, date of formal issuance (e.g., publication) of the distribution."@en ;
  skos:definition "En el contexto de DCAT 2.0 dcat:Distribution, fecha de emisión formal (es decir, publicación) de la distribución."@es ;
  skos:definition "V kontextu DCAT 2.0 dcat:Distribution, datum formálního vydání distribuce."@cs ;
  skos:definition "In the context of DCAT 2.0 dcat:Resource, date of formal issuance (e.g., publication) of the item."@en ;
  skos:definition "En el contexto de DCAT 2.0 dcat:Resource, fecha de emisión formal (es decir, publicación) de un ítem."@es ;
  skos:definition "V kontextu DCAT 2.0 dcat:Resource, datum formálního vydání položky."@cs ;
  skos:scopeNote "In the context of DCAT 2.0, this property SHOULD be set using the first known date of issuance."@en ;
  skos:scopeNote "En el contexto de DCAT 2.0, esta propiedad DEBERÍA incluir como valor la primer fecha de emisión."@es ;
  skos:scopeNote "V kontextu DCAT 2.0, tato vlastnost BY MĚLA obsahovat první známé datum vydání."@cs ;
  skos:scopeNote "In the context of DCAT 2.0 dcat:CatalogRecord, this indicates the date of listing the dataset in the catalog and not the publication date of the dataset itself."@en ;
  skos:scopeNote "En el contexto de DCAT 2.0 dcat:CatalogRecord, indica la fecha en que se lista el conjunto de datos en el catálogo, y no la fecha de publicación del propio conjunto de datos."@es ;
  skos:scopeNote "V kontextu DCAT 2.0 dcat:CatalogRecord, tato vlastnost indikuje datum zanesení datové sady do katalogu a ne datum vydání datové sady samotné."@cs ;
.
dct:language
  skos:definition "A language of the resource."@en ;
  skos:definition "In the context of DCAT 2.0, a language of the item. This refers to the natural language used for textual metadata (i.e. titles, descriptions, etc) of a catalogued resource (i.e. dataset or service) or the textual values of a dataset distribution."@en ;
  skos:definition "En el contexto de DCAT 2.0, el idioma del ítem. Este se refiere al lenguaje natural que se usa para los metadatos textuales (es decir, títulos, descripciones, etc) de un recurso catalogado (como ser un conjunto o servicio de datos) o los valores textuales de las distribuciones de un conjunto de datos."@es ;
  skos:definition "V kontextu DCAT 2.0, jazyk položky. Tato vlastnost úvádí přirozený jazyk použitý pro textová metadata, tj. názvy, popisy apod., katalogizovaného zdroje, tj. datové sady nebo služby, nebo textový obsah distribuce datové sady."@cs ;
  skos:scopeNote "In the context of DCAT 2.0, repeat this property if the resource is available in multiple languages."@en ;
  skos:scopeNote "En el contexto de DCAT 2.0, repetir esta propiedad si el recurso está disponible un múltiples idiomas."@es ;
  skos:scopeNote "V kontextu DCAT 2.0, tuto vlastnost opakujte, pokud je zdroj k dispozici ve více jazycích."@cs ;
  skos:scopeNote "In the context of DCAT 2.0, the value(s) provided for members of a catalog (i.e. dataset or service) override the value(s) provided for the catalog if they conflict."@en ;
  skos:scopeNote "En el contexto de DCAT 2.0, en el caso de conflictos, el valor (o los valores) datos para miembros del catálogo (es decir, conjunto de datos o servicios) sobreescribe el valor (o los valores) dados apra el catálogo."@es ;
  skos:scopeNote "V kontextu DCAT 2.0, hodnoty uvedené pro katalogizované položky, tj. datové sady či služby, mají přednost před hodnotami uvedenými pro katalog, pokud jsou ve sporu."@cs ;
  skos:scopeNote "In the context of DCAT 2.0, if representations of a dataset are available for each language separately, define an instance of dcat:Distribution for each language and describe the specific language of each distribution using dct:language (i.e. the dataset will have multiple dct:language values and each distribution will have just one as the value of its dct:language property)."@en;
  skos:scopeNote "En el contexto de DCAT 2.0, si las representaciones de un conjunto de datos están disponibles por separado para cada idioma, defina una instancia de dcat:Distribution para cada idioma y describa el lenguaje específico de cada distribución usando dct:language (es decir, el conjunto de datos tendrá múltiples valores para dct:language y cada distribución tendrá sólo un valor de la propiedad dct:language)."@es;
  skos:scopeNote "V kontextu DCAT 2.0, pokud jsou reprezentace datové sady k dispozici pro každý jazyk zvlášť, definujte pro každý jazyk jednu instanci dcat:Distribution a popište jazyk dané distribuce pomocí dct:language. (tj. datová sada bude mít více hodnot dct:language a každá distribuce bude mít pouze jednu hodnotu její vlastnosti dct:language)."@cs;
.
dct:license
  skos:definition "A legal document giving official permission to do something with the resource."@en ;
  skos:definition "In the context of DCAT 2.0 dcat:Resource, a legal document under which the resource is made available."@en ;
  skos:definition "En el contexto de DCAT 2.0 dcat:Resource, uh documento legal bajo el cuál se hace disponible el recurso."@es ;
  skos:definition "V kontextu DCAT 2.0 dcat:Resource, právní dokument popisující podmínky užití zdroje."@cs ;
  skos:definition "In the context of DCAT 2.0 dcat:Distribution, a legal document under which the distribution is made available."@en ;
  skos:definition "En el contexto de DCAT 2.0 dcat:Distribution, uh documento legal bajo el cuál se hace disponible la distribución."@es ;
  skos:definition "V kontextu DCAT 2.0 dcat:Distribution, právní dokument popisující podmínky užití distribuce."@cs ;
  skos:definition "In the context of DCAT 2.0 dcat:DataService, a legal document under which the service is made available."@en ;
  skos:definition "En el contexto de DCAT 2.0 dcat:DataService, uh documento legal bajo el cuál se hace disponible el servicio."@es ;
  skos:definition "V kontextu DCAT 2.0 dcat:DataService, právní dokument popisující podmínky užití služby."@cs ;
  skos:scopeNote "In the context of DCAT 2.0 dcat:Resource, information about licenses and rights MAY be provided for the Resource. See also guidance in the section 'License and rights statements'."@en ;
  skos:scopeNote "En el contexto de DCAT 2.0 dcat:Resource, PUEDE proveerse información sobre licencias y derechos para el Recurso. Vea también información en la sección 'License and rights statements'."@es ;
  skos:scopeNote "V kontextu DCAT 2.0 dcat:Resource, pro Zdroj MŮŽE BÝT uvedena informace o podmínkách užití (licencích a právech). Viz návod v sekci 'License and rights statements'."@cs ;
  skos:scopeNote "In the context of DCAT 2.0, information about licenses and rights SHOULD be provided on the level of Distribution. Information about licenses and rights MAY be provided for a Dataset in addition to but not instead of the information provided for the Distributions of that Dataset. Providing license or rights information for a Dataset that is different from information provided for a Distribution of that Dataset SHOULD be avoided as this can create legal conflicts. See also guidance in the section 'License and rights statements'."@en ;
  skos:scopeNote "En el contexto de DCAT 2.0, la información sobre licencias y derechos DEBERÍA darse a nivel de la Distribución. La información sobre licencias y derechos PUEDE proveerse también para un conjunto de datos pero no en lugar de la información para la distribución del conjunto de datos. Se DEBERÍA evitar dar información de licencia o derechos para un conjunto de datos que es diferente de la de su distribución ya que en este caso puede haber conflictos legales. Ver más información en la sección 'License and rights statements'."@es ;
  skos:scopeNote "V kontextu DCAT 2.0, informace o podmínkách užití (licencích a právech) BY MĚLY být poskytnuty na úrovni distribuce. Navíc, nikoliv místo, MOHOU BÝT informace o podmínkách užití (licencích a právech) poskytnuty na úrovni datové sady. NEMĚLY BY SE poskytnout různé podmínky užití pro datovou sadu a pro její distribuci, jelikož to může vést ke sporům v právním výkladu. Viz také návod v sekci 'License and rights statements'."@cs ;
.
dct:modified
  skos:definition "Date on which the resource was changed."@en ;
  skos:definition "In the context of DCAT 2.0 dcat:Resource, most recent date on which the item was changed, updated or modified."@en ;
  skos:definition "En el contexto de DCAT 2.0 dcat:Resource, la fecha más reciente en la que se modificó o actualizó el ítem del catálogo."@es ;
  skos:definition "V kontextu DCAT 2.0 dcat:Resource, poslední datum kdy byla položka změněna či aktualizována."@cs ;
  skos:definition "In the context of DCAT 2.0 dcat:Distribution, most recent date on which the distribution  was changed, updated or modified."@en ;
  skos:definition "En el contexto de DCAT 2.0 dcat:Distribution, la fecha más reciente en la que se modificó o actualizó la distribución."@es ;
  skos:definition "V kontextu DCAT 2.0 dcat:Distribution, poslední datum kdy byla distribuce změněna či aktualizována."@cs ;
  skos:definition "In the context of DCAT 2.0 dcat:CatalogRecord, most recent date on which the catalog entry was changed, updated or modified."@en ;
  skos:definition "En el contexto de DCAT 2.0 dcat:CatalogRecord, la fecha más reciente en la que se modificó o actualizó la entrada del catálogo."@es ;
  skos:definition "V kontextu DCAT 2.0 dcat:CatalogRecord, poslední datum kdy byl katalogizační záznam změněn či aktualizován."@cs ;
  skos:scopeNote "In the context of DCAT 2.0 dcat:Resource, the value of this property indicates a change to the actual item, not a change to the catalog record. An absent value MAY indicate that the item has never changed after its initial publication, or that the date of last modification is not known, or that the item is continuously updated."@en ;
  skos:scopeNote "En el contexto de DCAT 2.0 dcat:Resource, el valor de esta propiedad indica un cambio del ítem, no un cambio en el registro del catálogo. La ausencia de valor PUEDE indicar que el ítem nunca se modificó después de su publicación inicial, o que no se conoce la fecha de su última modificación, o que el ítem se actualiza contínuamente."@es ;
  skos:scopeNote "V kontextu DCAT 2.0 dcat:Resource, hodnota této vlastnosti udává změnu položky, nikoliv změnu jejího katalogizačního záznamu. Pokud hodnota chybí, MŮŽE to znamenat, že po publikaci položka již nebyla měněna, že datum změny není známo, nebo že je položka aktualizována neustále."@cs ;
  skos:scopeNote "In the context of DCAT 2.0 dcat:CatalogRecord, this indicates the date of last change of a catalog entry, i.e. the catalog metadata description of the dataset, and not the date of the dataset itself."@en ;
  skos:scopeNote "En el contexto de DCAT 2.0 dcat:CatalogRecord, indica la fecha en que se hizo la última modificación a la entrada del catálogo, es decir, de los metadatos en el catálogo sobre el conjunto de datos, y no sobre el mismo conjunto de datos."@es ;
  skos:scopeNote "V kontextu DCAT 2.0 dcat:CatalogRecord, tato vlastnost indikuje datum poslední změny katalogizačního záznamu, nikoliv datum změny datové sady samotné."@cs ;
.
dct:publisher
  skos:definition "An entity responsible for making the resource available."@en ;
  skos:definition "In the context of DCAT 2.0, the entity responsible for making the item available."@en ;
  skos:definition "En el contexto de DCAT 2.0, la entidad responsable de hacer el item disponible."@es ;
  skos:definition "V kontextu DCAT 2.0, entita zodpovědná za zpřístupnění položky."@cs ;
  skos:scopeNote "In the context of DCAT 2.0, resources of type foaf:Agent are recommended as values for this property."@en ;
  skos:scopeNote "En el contexto de DCAT 2.0, se recomienda usar recursos del tipo foaf:Agent para los valores de esta propiedad."@es ;
  skos:scopeNote "V kontextu DCAT 2.0, doporučovanou hodnotou této vlastnosti jsou zdroje typu foaf:Agent."@cs ;
.
dct:relation
  skos:definition "A related resource."@en ;
  skos:definition "In the context of DCAT 2.0 dcat:Resource, a resource with an unspecified relationship to the catalogued item."@en ;
  skos:definition "En el contexto de DCAT 2.0 dcat:Resource, un recurso con una relación no especificada con el recurso catalogado que se está describiendo."@es ;
  skos:definition "V kontextu DCAT 2.0 dcat:Resource, Zdroj s nespecifikovaným vztahem ke katalogizované položce."@cs ;
  skos:definition "In the context of DCAT 2.0 dcat:Relationship, the resource related to the source resource."@en ;
  skos:definition "En el contexto de DCAT 2.0 dcat:Relationship, el recurso relacionado con el recurso que se está describiendo."@es ;
  skos:definition "V kontextu DCAT 2.0 dcat:Relationship, Zdroj ve vztahu se popisovaným zdrojem."@cs ;
  skos:scopeNote "In the context of a DCAT 2.0 dcat:Relationship this is expected to point to another dcat:Dataset or other catalogued resource"@en ;
  skos:scopeNote "V kontextu DCAT 2.0 dcat:Relationship se očekává, že tato vlastnost bude ukazovat na jiný dcat:Dataset nebo jiný katalogizovaný zdroj"@cs ;
  skos:scopeNote "In the context of DCAT 2.0, see also: Sub-properties of dct:relation in particular dcat:distribution, dct:hasPart, dct:isPartOf, dct:conformsTo, dct:isFormatOf, dct:hasFormat, dct:isVersionOf, dct:hasVersion, dct:replaces, dct:isReplacedBy, dct:references, dct:isReferencedBy, dct:requires, dct:isRequiredBy"@en ;
  skos:scopeNote "V kontextu DCAT 2.0, viz také: Podvlastnosti dct:relation, zejména dcat:distribution, dct:hasPart, dct:isPartOf, dct:conformsTo, dct:isFormatOf, dct:hasFormat, dct:isVersionOf, dct:hasVersion, dct:replaces, dct:isReplacedBy, dct:references, dct:isReferencedBy, dct:requires, dct:isRequiredBy"@cs ;
  skos:scopeNote "In the context of DCAT 2.0, dct:relation SHOULD be used where the nature of the relationship between a catalogued item and related resources is not known. A more specific sub-property SHOULD be used if the nature of the relationship of the link is known. The property dcat:distribution SHOULD be used to link from a dcat:Dataset to a representation of the dataset, described as a dcat:Distribution"@en ;
  skos:scopeNote "V kontextu DCAT 2.0, dct:relation BY MĚLA být použita tam, kde není znám typ vztahu mezi katalogizovanou položkou a vztaženým zdrojem. Pokud typ vztahu znám je, MĚLA BY být použita konkrétnější podvlastnost. Pro propojení datové sady dcat:Dataset a reprezentaci datové sady dcat:Distribution BY MĚLA BÝT použita vlastnost dcat:distribution."@cs ;
.
dct:rights
  skos:definition "Information about rights held in and over the resource."@en ;
  skos:definition "In the context of DCAT 2.0 dcat:Resource, a statement that concerns all rights not addressed with dct:license or dct:accessRights, such as copyright statements."@en ;
  skos:definition "En el contexto de DCAT 2.0 dcat:Resource, una declaración que tiene que ver con todos los derechos no representados con dct:license o dct:accessRights, como por ejemplo declaraciones de derechos de autor."@es ;
  skos:definition "V kontextu DCAT 2.0 dcat:Resource, dokument zabývající se všemi právy, které nejsou ošetřeny v dct:license či dct:rights, jako je například copyright."@cs ;
  skos:definition "In the context of DCAT 2.0 dcat:Distribution, information about rights held in and over the distribution."@en ;
  skos:definition "En el contexto de DCAT 2.0 dcat:Distribution, información sobre los derechos mantenido por las distribuciones."@es ;
  skos:definition "V kontextu DCAT 2.0 dcat:Distribution, informace o právech vztahujících se na distribuci."@cs ;
  skos:scopeNote "In the context of DCAT 2.0, information about licenses and rights MAY be provided for the Resource. See also guidance in the section 'License and rights statements'."@en ;
  skos:scopeNote "En el contexto de DCAT 2.0, información sobre licencias y derechos PUEDE proveerse para un Recurso. Ver también la sección 'License and rights statements' para más información."@es ;
  skos:scopeNote "V kontextu DCAT 2.0, pro Zdroj MŮŽE BÝT uvedena informace o podmínkách užití (licencích a právech). Viz návod v sekci 'License and rights statements'."@cs ;
  skos:scopeNote """In the context of DCAT 2.0 dcat:Distribution, dct:license, which is a sub-property of dct:rights, can be used to link a distribution to a license document. However, dct:rights allows linking to a rights statement that can include licensing information as well as other information that supplements the license such as attribution.
Information about licenses and rights SHOULD be provided on the level of Distribution. Information about licenses and rights MAY be provided for a Dataset in addition to but not instead of the information provided for the Distributions of that Dataset. Providing license or rights information for a Dataset that is different from information provided for a Distribution of that Dataset SHOULD be avoided as this can create legal conflicts. See also guidance in the secion on 'License and rights statements'."""@en ;
  skos:scopeNote """En el contexto de DCAT 2.0 dcat:Distribution, dct:license, que es una sub-propertiedad de dct:rights, puede usarse para asociar una distribución a un documento de licencia. Sin embargo, dct:rights permite asociar a una declaración de derechos que incluya información de licencias así como también otra información que suplementa la licencia, como atribución.
La información sobre las licencias y derechos DEBERÍA proveerse a nivel de la Distribución. La información sobre licencias y derechos PUEDE proveerse también para un conjunto de datos pero no en lugar de la información provista para las Distribuciones del conjunto de datos. Se DEBERÍA evitar brindar información sobre licencias y derechos de un conjunto de datos que difiere de aquella de la Distribución del conjunto de datos ya que se crean conflictos legales. Ver también la sección 'License and rights statements' para más información."""@es ;
  skos:scopeNote """V kontextu DCAT 2.0 dcat:Distribution, dct:license, což je podvlastnost dct:rights, může být použita k propojení distribuce a licenčního dokumentu. dct:rights ale umožňuje odkazovat na podmínky užití, které také mohou obsahovat licenční informace, které mohou licenci upřesňovat například nutností citace.
Informace o podmínkách užití (licencích a právech) BY MĚLY být poskytnuty na úrovni distribuce. Navíc, nikoliv místo, MOHOU BÝT informace o podmínkách užití (licencích a právech) poskytnuty na úrovni datové sady. NEMĚLY BY SE poskytnout různé podmínky užití pro datovou sadu a pro její distribuci, jelikož to může vést ke sporům v právním výkladu. Viz také návod v sekci 'License and rights statements'."""@cs ;
.
dct:spatial
  skos:definition "Spatial characteristics of the resource."@en ;
  skos:definition "In the context of DCAT 2.0 dcat:Dataset, the geographical area covered by the dataset."@en ;
  skos:definition "En el contexto de DCAT 2.0 dcat:Dataset, el área geográfica cubierta por el conjunto de datos."@es ;
  skos:definition "V kontextu DCAT 2.0 dcat:Dataset, geografické území pokryté datovou sadou."@cs ;
  skos:scopeNote "In the context of DCAT 2.0 dcat:Dataset, the spatial coverage of a dataset may be encoded as an instance of dct:Location, or may be indicated using a URI reference (link) to a resource describing a location. It is recommended that links are to entries in a well maintained gazetteer such as Geonames."@en ;
  skos:scopeNote "En el contexto de DCAT 2.0 dcat:Dataset, la cobertura espacial de un conjunto de datos puede codificarse como una instancia de dct:Location, o puede indicarse usando una referencia URI (es decir, un enlace) a un recurso que describa la posición. Se recomienda que los enlaces sean a entradas en un diccionario geográfico bien mantenido como Geonames."@es ;
  skos:scopeNote "V kontextu DCAT 2.0 dcat:Dataset, územní pokrytí datové sady může být zaznamenáno jako instance dct:Location, nebo může být indikováno jako IRI odkazující na zdroj popisující území. Je doporučeno se odkazovat na udržovaný zdroj dat jako například Geonames."@cs ;
.
dct:temporal
  skos:definition "Temporal characteristics of the resource."@en ;
  skos:definition "In the context of DCAT 2.0 dcat:Dataset, the temporal period that the dataset covers."@en ;
  skos:definition "En el contexto de DCAT 2.0 dcat:Dataset, el período temporal cubierto por el conjunto de datos."@es ;
  skos:definition "V kontextu DCAT 2.0 dcat:Dataset, časové pokrytí datové sady."@cs ;
  skos:scopeNote "In the context of DCAT 2.0 dcat:Dataset, the temporal coverage of a dataset may be encoded as an instance of dct:PeriodOfTime, or may be indicated using a URI reference (link) to a resource describing a time period or interval."@en ;
  skos:scopeNote "En el contexto de DCAT 2.0 dcat:Dataset, la cobertura temporal del conjunto de datos puede codificarse como una instancia de dct:PeriodOfTime, o puede indicarse usando una referencia URI (es decir, un enlace) a un recurso que describa el período o interválo de tiempo."@es ;
  skos:scopeNote "V kontextu DCAT 2.0 dcat:Dataset, časové pokrytí datové sady může být zaznamenáno jako instance dct:PeriodOfTime, nebo může být indikováno jako IRI odkazující na zdroj popisující či časový interval."@cs ;
.
dct:title
  skos:definition "A name given to the resource."@en ;
  skos:definition "In the context of DCAT 2.0 dcat:Resource, a name given to the item."@en ;
  skos:definition "En el contexto de DCAT 2.0 dcat:Resource, un nombre o título dado al elemento del catálogo."@es ;
  skos:definition "V kontextu DCAT 2.0 dcat:Resource, název položky"@cs ;
  skos:definition "In the context of DCAT 2.0 dcat:Distribution, a name given to the distribution."@en ;
  skos:definition "En el contexto de DCAT 2.0 dcat:Distribution, un nombre o título dado a la distribución."@en ;
  skos:definition "V kontextu DCAT 2.0 dcat:Distribution, název distribuce"@cs ;
.
dct:type
  skos:definition "The nature or genre of the resource."@en ;
  skos:definition "La naturaleza, género o tipo del recurso."@es ;
  skos:definition "Podstata či žánr zdroje."@cs ;
  skos:scopeNote """In the context of DCAT 2.0, the value SHOULD be taken from a well governed and broadly recognised controlled vocabulary, such as:
1. DCMI Type vocabulary [DCTERMS]
2. ISO 19115 scope codes [ISO-19115-1]
3. Datacite resource types [DataCite]
4. PARSE.Insight content-types used by re3data.org [RE3DATA-SCHEMA] (see item 15 contentType)
5. MARC intellectual resource types
Some members of these controlled vocabularies are not strictly suitable for datasets or data services (e.g. DCMI Type Event, PhysicalObject; ISO 19115 CollectionHardware, CollectionSession, Initiative, Sample, Repository), but might be used in the context of other kinds of catalogs defined in DCAT profiles or applications."""@en ;
  skos:scopeNote """En el contexto de DCAT 2.0, el valor DEBERÍA tomarse de un vocabulario controlado bien gobernado y ampliamente reconocido, como por ejemplo:
1. DCMI Type vocabulary [DCTERMS]
2. códigos de alcance de ISO 19115 [ISO-19115-1]
3. tipos de recursos de Datacite [DataCite]
4. tipos de contenido de PARSE.Insight usados por re3data.org [RE3DATA-SCHEMA] (see item 15 contentType)
5. tipos de recurso intelectual de MARC
Algunos elementos de estos vocabularios controlados son estrictamente no apropiados para conjuntos de datos o servicios de datos (por ejemplo: DCMI Type Event, PhysicalObject; ISO 19115 CollectionHardware, CollectionSession, Initiative, Sample, Repository), pero pueden usarse en este contexto para otros tipos de catálogos definidos en perfiles de DCAT o aplicaciones."""@es ;
  skos:scopeNote """V kontextu DCAT 2.0, hodnota BY MĚLA být z dobře řízeného a široce uznávaného slovníku, např.:
1. Slovník DCMI Type [DCTERMS]
2. Kódy ISO 19115 [ISO-19115-1]
3. Typy zdrojů Datacite [DataCite]
4. Typy obsahu PARSE.Insight, které jsou používány re3data.org [RE3DATA-SCHEMA] (viz položka 15 contentType)
5. Typy duševních zdrojů MARC
Některé položky těchto slovníků nejsou zcela vhodné pro datové sady nebo datové služby (např. DCMI Type Event, PhysicalObject; ISO 19115 CollectionHardware, CollectionSession, Initiative, Sample, Repository), ale mohou být použity v kontextu jiných typů katalogů, které jsou definovány v profilech či aplikacích DCAT."""@cs ;
  skos:scopeNote "To describe the file format, physical medium, or dimensions of the resource, use the dct:format element."@en ;
  skos:scopeNote "Usa el elemento dct:format para describir el formato del archivo, el medio físico, o las dimensiones del recurso."@es ;
  skos:scopeNote "Pro popis formátu souboru, fyzického média či dimenzí zdroje použijte dct:format."@cs ;
.
foaf:homepage
  rdf:type owl:ObjectProperty ; # needed so OWLAPI doesn't choke
  skos:definition "A homepage for some thing."@en ;
  skos:definition "In the context of DCAT 2.0 dcat:Catalog, a homepage of the catalog (a public Web document usually available in HTML)."@en ;
  skos:scopeNote "foaf:homepage is an inverse functional property (IFP), which means that it MUST be unique and precisely identify the web-page for the resource. In the context of DCAT 2.0, this property indicates the canonical web-page, which might be helpful in cases where there is more than one web-page about the resource."@en ;
  skos:scopeNote "foaf:homepage es la propiedad funcional inversa (IFP por sus siglas en inglés), lo que significa que DEBE ser única y identificar la página web del recurso percisamente. En el contexto de DCAT 2.0, esta propiedad indica la página web canónica, que pude ser útil en casos en los que hay más de una página web para el recurso."@es ;
  skos:scopeNote "foaf:homepage je inverzní funkčí vlastnost, což znamená, že MUSÍ být unikátní a MUSÍ přesně označovat webovou stránku zdroje. V kontextu DCAT 2.0, označuje hlavní webovou stránku, což se může hodit v případě, že webových stránek o zdroji existuje více."@cs ;
.
foaf:primaryTopic
  rdf:type owl:ObjectProperty ; # needed so OWLAPI doesn't choke
  skos:definition "The primary topic of some page or document."@en ;
  skos:definition "In the context of DCAT 2.0 dcat:CatalogRecord, the dcat:Resource (dataset or service) described in the record."@en ;
  skos:definition "En el contexto de DCAT 2.0 dcat:CatalogRecord, el dcat:Resource (conjunto de datos o servicio) descripto en el registro."@es ;
  skos:definition "V kontextu DCAT 2.0 dcat:CatalogRecord, dcat:Resource (datová sada či služba) popsaná katalogizačním záznamem."@cs ;
  skos:scopeNote "foaf:primaryTopic property is functional: in the context of DCAT 2.0, each catalog record can have at most one primary topic i.e. describes one dataset or service."@en ;
  skos:scopeNote "La propiedad foaf:primaryTopic es funcional: en el contexto de DCAT 2.0,  cada registro del catálogo puede tener a lo sumo un tópico principal, es decir un tópico que describa el conjunto de datos o servicio."@es ;
  skos:scopeNote "Vlastnost foaf:primaryTopic je funkce: v kontextu DCAT 2.0, každý katalogizační záznam může mít nejvýše jednu hodnotu foaf:primaryTopic, tj. popisuje nejvýše jednu datovou sadu či službu."@cs ;
.
odrl:hasPolicy
  skos:editorialNote "Czech translation to be updated"@en ;
	skos:definition "Identifies an ODRL Policy for which the identified Asset is the target Asset to all the Rules."@en ;
  skos:definition "In the context of DCAT 2.0 dcat:Resource, an ODRL conformant policy expressing the rights associated with the resource."@en ;
  skos:definition "Nel contesto di DCAT 2.0 dcat:Resource, una policy conforme all'ODRL che esprime i diritti associati alla risorsa."@it ;
  skos:definition "En el contexto de DCAT 2.0 dcat:Resource, una reglamentación conforme a ODRL expresando los derechos asociados con el recurso [ODRL-VOCAB]."@es ;
  skos:definition "V kontextu DCAT 2.0 dcat:Resource, pravidlo vyjadřující práva spojená se zdrojem, pokud je použit slovník ODRL [ODRL-VOCAB]."@cs ;
  skos:definition "In the context of DCAT 2.0 dcat:Distribution, an ODRL conformant policy expressing the rights associated with the distribution."@en ;
  skos:definition "Nel contesto di DCAT 2.0 dcat:Distribution, una policy conforme all'ODRL che esprime i diritti associati alla distribuzione."@it ;
  skos:definition "En el contexto de DCAT 2.0 dcat:Distribution, una reglamentación conforme a ODRL expresando los derechos asociados con la distribución [ODRL-VOCAB]."@es ;
  skos:definition "V kontextu DCAT 2.0 dcat:Distribution, pravidlo vyjadřující práva spojená s distribucí, pokud je použit slovník ODRL [ODRL-VOCAB]."@cs ;
  skos:scopeNote "In the context of DCAT 2.0 dcat:Resource, information about rights expressed as an ODRL policy [ODRL-MODEL] using the ODRL vocabulary [ODRL-VOCAB] MAY be provided for the resource. See also guidance at the section 'License and rights statements'."@en ;
  skos:scopeNote "Nel contesto DCAT 2.0 dcat:Resource, le informazioni sui diritti espressi come policy ODRL [ODRL-MODEL] utilizzando il vocabolario ODRL [ODRL-VOCAB] POSSONO essere fornite per la risorsa. Si veda anche la guida alla sezione 'Licenza e dichiarazioni sui diritti'."@it ;
  skos:scopeNote "En el contexto de DCAT 2.0 dcat:Resource, información sobre los derechos expresados como reglamentación ODRL [ODRL-MODEL] usando el vocabulario ODRL [ODRL-VOCAB] PUEDE proveerse para el Recurso. Ver también la información en la sección 'License and rights statements.'"@es ;
  skos:scopeNote "V kontextu DCAT 2.0 dcat:Resource, pro zdroj MŮŽE BÝT uvedena informace o právech vyjádřená pomocí pravidel slovníku ODRL [ODRL-VOCAB]. Viz také návod v sekci 'License and rights statements'."@cs ;
  skos:scopeNote "In the context of DCAT 2.0 dcat:Distribution, information about rights expressed as an ODRL policy [ODRL-MODEL] using the ODRL vocabulary [ODRL-VOCAB] MAY be provided for the distribution. See also guidance at the section 'License and rights statements'."@en ;
  skos:scopeNote "Nel contesto di DCAT 2.0 dcat:Distribution, le informazioni sui diritti espressi come policy ODRL [ODRL-MODEL] utilizzando il vocabolario ODRL [ODRL-VOCAB] POSSONO essere fornite per la distribuzione. Si veda anche la guida alla sezione 'Licenza e dichiarazioni sui diritti'."@it ;
  skos:scopeNote "En el contexto de DCAT 2.0 dcat:Distribution, información sobre los derechos expresados como reglamentación ODRL [ODRL-MODEL] using the ODRL vocabulary [ODRL-VOCAB] PUEDE proveerse para el Distribución. Ver también la información en la sección 'License and rights statements.'"@es ; 
  skos:scopeNote "V kontextu DCAT 2.0 dcat:Distribution, pro distribuci MŮŽE BÝT uvedena informace o právech vyjádřená pomocí pravidel slovníku ODRL [ODRL-VOCAB]. Viz také návod v sekci 10. 'License and rights statements'."@cs ;
 .

prov:qualifiedAttribution
  skos:definition "In the context of DCAT 2.0, link to an Agent having some form of responsibility for the resource."@en ;
  skos:definition "En el contexto de DCAT 2.0, enlace a un Agente que tiene alguna forma de responsabilidad con el recurso."@es ;
  skos:definition "Nel contesto di DCAT 2.0, collegamento a un agente che ha una qualche forma di responsabilità per la risorsa"@it ;
  skos:definition "V kontextu DCAT 2.0, odkaz na Agenta, který má nějaký typ odpovědnosti za zdroj."@cs ;
  skos:scopeNote """In the context of DCAT 2.0, used to link to an Agent where the nature of the relationship is known but does not match one of the standard Dublin Core properties (dct:creator, dct:publisher).
  Use dcat:hadRole on the prov:Attribution to capture the responsibility of the Agent with respect to the Resource. See https://w3c.github.io/dxwg/dcat/#qualified-attribution for usage examples."""@en ;
  skos:scopeNote """En el contexto de DCAT 2.0, se usa para asociar un Agente cuando la naturaleza de la relación es conocida pero no es ninguna de las asociaciones estándares descriptas con propiedades de Dublin Core (dct:creator, dct:publisher).
    Se usa dcat:hadRole en la prov:Attribution para capturar la responsabilidad del Agente con respecto al Recurso. Ver https://w3c.github.io/dxwg/dcat/#qualified-attribution para más ejemplos de uso."""@es ;
  skos:scopeNote "Nel contesto di DCAT 2.0, utilizzato per collegarsi a un agente in cui la natura della relazione è nota ma non corrisponde a una delle proprietà Dublin Core standard (dct: creatore, dct: editore). Si usi dcat:hadRole su prov:Attribution per rappresentare la responsabilità dell'Agente in relazione alla Risorsa. Si veda https://w3c.github.io/dxwg/dcat/#qualified-attribution per gli esempi di utilizzo."@it;
  skos:scopeNote """V kontextu DCAT 2.0, vlastnost se používá pro odkaz na Agenta tam, kde typ vztahu je znám, ale neodpovídá žádné ze standardních vlastností Dublin Core (dct:creator, dct:publisher).
  Pro reprezentaci vztahu Agenta ke zdroji použijte vlastnost dcat:hadRole na třídě prov:Attribution. Viz  https://w3c.github.io/dxwg/dcat/#qualified-attribution pro příklady užití."""@cs ;
  skos:changeNote "Property added in this context in DCAT 2.0."@en ;
  skos:changeNote "Esta propiedad fue agregada en DCAT 2.0."@es ;
  skos:changeNote "Vlastnost v tomto kontextu byla přidána ve verzi DCAT 2.0"@cs ;
.
prov:wasGeneratedBy
  rdfs:subPropertyOf dct:relation ;
  skos:definition "In the context of DCAT 2.0 dcat:Dataset, an activity that generated, or provides the business context for, the creation of the dataset."@en ;
  skos:scopeNote "In the context of DCAT 2.0 dcat:Dataset, the activity associated with generation of a dataset will typically be an initiative, project, mission, survey, on-going activity ('business as usual') etc. Multiple prov:wasGeneratedBy properties can be used to indicate the dataset production context at various levels of granularity."@en ;
  skos:scopeNote "En el contexto de DCAT 2.0 dcat:Dataset, la actividad asociada con la generación de un conjunto de datos. Típicamente es una iniciativa, proyecto, misión, encuensta, una actividad contínua (la actividad usual) etc. Se pueden usar múltiples propiedades  prov:wasGeneratedBy para indicar el contexto de producción del conjunto de datos en disintos niveles de granularidad."@es ;
  skos:scopeNote "V kontextu DCAT 2.0 dcat:Dataset, aktivitou spojenou s tvorbou datové sady typicky bývá iniciativa, projekt, mise, rešerše, průběžná aktivita (běžný chod podniku) apod. Pro zaznamenání kontextu datové sady na více úrovních granulariy lze použít více hodnot vlastnosti prov:wasGeneratedBy."@cs ;
  skos:scopeNote "In the context of DCAT 2.0 dcat:Dataset, use prov:qualifiedGeneration to attach additional details about the relationship between the dataset and the activity, e.g. the exact time that the dataset was produced during the lifetime of a project."@en ;
  skos:scopeNote "En el contexto de DCAT 2.0 dcat:Dataset, utiliza prov:qualifiedGeneration para adjuntar detalles adicionales sobre la relación entre el conjunto de datos y la actividad activity, por ejemplo, el tiempo exacto en el que se produjo el conjunto de datose durante la vida de un proyecto."@es ;
  skos:scopeNote "V kontextu DCAT 2.0 dcat:Dataset, pro připojení podrobností o vztahu mezi datovou sadou a aktivitou, např. přesný čas kdy byla datová sada vyprodukována během životního cyklu projektu, použijte prov:qualifiedGeneration."@cs ;
  skos:changeNote "Property added in this context in DCAT 2.0."@en ;
  skos:changeNote "Esta propiedad fue agregada en DCAT 2.0."@es ;
  skos:changeNote "Vlastnost v tomto kontextu byla přidána ve verzi DCAT 2.0"@cs ;

.
prov:wasAttributedTo
  rdfs:subPropertyOf dct:relation ;
.
prov:wasDerivedFrom
  rdfs:subPropertyOf dct:relation ;
.
prov:wasInfluencedBy
  rdfs:subPropertyOf dct:relation ;
.
prov:wasQuotedFrom
  rdfs:subPropertyOf dct:relation ;
.
prov:wasRevisionOf
  rdfs:subPropertyOf dct:relation ;
.
prov:hadPrimarySource
  rdfs:subPropertyOf dct:relation ;
.
prov:alternateOf
  rdfs:subPropertyOf dct:relation ;
.
prov:specializationOf
  rdfs:subPropertyOf dct:relation ;
.
time:hasBeginning
  skos:definition "Beginning of a temporal entity."@en ;
  skos:definition "In the context of DCAT 2.0, beginning of a period or interval."@en ;
  skos:scopeNote "In the context of DCAT 2.0, use of the property time:hasBeginning entails that value of the dct:temporal property is a member of the time:TemporalEntity class from [OWL-TIME]. In this context this could be taken to imply that dct:PeriodOfTime is equivalent to the subclass time:ProperInterval"@en ;
  skos:scopeNote "En el contexto de DCAT 2.0, el uso de la propiedad time:hasBeginning implica que el valor de la propiedad dct:temporal es un miembro de la clase time:TemporalEntity de [OWL-TIME]. En este contexto, esto puede interpretarse como que implica que dct:PeriodOfTime es equivalente a la subclase time:ProperInterval"@es ;
  skos:scopeNote "V kontextu DCAT 2.0, použití vlastnosti time:hasBeginning znamená, že hodnota vlastnosti dct:temporal je instancí třídy time:TemporalEntity ze slovníku [OWL-TIME]. V tomto kontextu to může znamenat, že dct:PeriodOfTime je ekvivalentní podtřídě time:ProperInterval"@cs ;
  skos:changeNote "Property added in this context in DCAT 2.0."@en ;
  skos:changeNote "Esta propiedad fue agregada en DCAT 2.0."@es ;
  skos:changeNote "Vlastnost v tomto kontextu byla přidána ve verzi DCAT 2.0"@cs ;
.
time:hasEnd
  skos:definition "End of a temporal entity."@en ;
  skos:definition "In the context of DCAT 2.0, end of a period or interval."@en ;
  skos:scopeNote "In the context of DCAT 2.0, use of the property time:hasEnd entails that value of the dct:temporal property is a member of the time:TemporalEntity class from [OWL-TIME]. In this context this could be taken to imply that dct:PeriodOfTime is equivalent to the subclass time:ProperInterval"@en ;
  skos:scopeNote "En el contexto de DCAT 2.0, el uso de la propiedad time:hasEnd implica que el valor de la propiedad dct:temporal es un miembro de la clase time:TemporalEntity de [OWL-TIME]. En este contexto, esto puede interpretarse como que implica que dct:PeriodOfTime es equivalente a la subclase time:ProperInterval"@es ;
  skos:scopeNote "V kontextu DCAT 2.0, použití vlastnosti time:hasEnd znamená, že hodnota vlastnosti dct:temporal je instancí třídy time:TemporalEntity ze slovníku [OWL-TIME]. V tomto kontextu to může znamenat, že dct:PeriodOfTime je ekvivalentní podtřídě time:ProperInterval"@cs ;
  skos:changeNote "Property added in this context in DCAT 2.0."@en ;
  skos:changeNote "Esta propiedad fue agregada en DCAT 2.0."@es ;
  skos:changeNote "Vlastnost v tomto kontextu byla přidána ve verzi DCAT 2.0"@cs ;
.
locn:geometry
  rdfs:range rdfs:Literal ;
  skos:definition "Associates any resource with the corresponding geometry."@en ;
  skos:definition "Asocia cualquier recurso con la geometría correspondiente."@es ;
  skos:definition "Přiřazuje geometrii jakémukoliv zdroji."@cs ;
  skos:scopeNote "In the context of DCAT 2.0, the range of this property is intentionally generic, with the purpose of allowing different geometry encodings. E.g., the geometry could be encoded as WKT (geosparql:asWKT [GeoSPARQL])."@en ;
  skos:scopeNote " el contexto de DCAT 2.0, el rango de esta propiedad es intencionalmente genérico con el propósito de permitir distintas codificaciones de la geometría. Por ejemplo, la geometría puede codificarse como WKT (geosparql:asWKT [GeoSPARQL])."@es ;
  skos:scopeNote "V kontextu DCAT 2.0, obor hodnot této vlastnosti je úmyslně obecný, aby umožnil různé kódování geometrií. Geometrie by kupříkladu mohla být kódována jako WKT (geosparql:asWKT [GeoSPARQL])"@cs ;
  skos:changeNote "Property added in this context in DCAT 2.0."@en ;
  skos:changeNote "Esta propiedad fue agregada en DCAT 2.0."@es ;
  skos:changeNote "Vlastnost v tomto kontextu byla přidána ve verzi DCAT 2.0"@cs ;
.
